- Added ASR_THM and ROR_THM - Made use of MOD_TIMES2 - Tidied up a bit

src/word32/bitsScript.sml
@@ -1,16 +1,17 @@
-(* app load ["bossLib"]; *)
-open HolKernel boolLib Parse Q bossLib simpLib numLib
-     pairTheory numeralTheory arithmeticTheory prim_recTheory;
+(* app load ["bossLib","abbrevUtil"]; *)
+open HolKernel boolLib abbrevUtil Q Parse bossLib simpLib
+     numLib pairTheory numeralTheory arithmeticTheory prim_recTheory;
 
 infix 8 by;
-infix THEN THENC THENL ++;
+infix THEN THENC THENL ++ |->;
  
-
 (* -------------------------------------------------------- *)
 
 val _ = new_theory "bits";
 
 (* -------------------------------------------------------- *)
+
+val DIV2_def        = Define `DIV2 n = n DIV 2`;
 
 val TIMES_2EXP_def  = Define `TIMES_2EXP x n = n * 2 EXP x`;
 
@@ -31,236 +32,284 @@ val SLICE_def       = Define `SLICE h l n = MOD_2EXP (SUC h) n - MOD_2EXP l n`;
 val LSB_def         = Define `LSB = BIT 0`;
 
 val BITWISE_def =
- Define
-   `(BITWISE 0 op x y = 0)
- /\ (BITWISE (SUC n) op x y =
+  Define`
+     (BITWISE 0 op x y = 0)
+  /\ (BITWISE (SUC n) op x y =
          BITWISE n op x y + SET (op (BIT n x) (BIT n y)) n)`;
 
 (* -------------------------------------------------------- *)
 (* -------------------------------------------------------- *)
 
-val ZERO_LT_TWOEXP = save_thm("ZERO_LT_TWOEXP",
-  GEN_ALL (REDUCE_RULE (Q.SPECL [`n`,`1`] ZERO_LESS_EXP))
-);
-
-val BITS_THM = save_thm("BITS_THM",
-   REWRITE_RULE [DIV_2EXP_def,MOD_2EXP_def] BITS_def
-);
-
-val BITSLT_THM = Q.store_thm("BITSLT_THM",
-  `!h l n. BITS h l n < 2 EXP (SUC h-l)`,
-  RW_TAC std_ss [BITS_THM,ZERO_LT_TWOEXP,DIVISION]
-);
-
-val DIV_MULT_LEM = Q.store_thm("DIV_MULT_LEM",
-  `!m n. 0 < n ==> m DIV n * n <= m`,
-  RW_TAC arith_ss [LESS_EQ_EXISTS]
-    THEN Q.EXISTS_TAC `m MOD n`
-    THEN PROVE_TAC [DIVISION,ADD_COMM]
-);
- 
-val DIV_MULT_LESS_EQ = 
-  GEN_ALL (SIMP_RULE std_ss [ZERO_LT_TWOEXP] 
-             (Q.SPECL [`n`,`2 EXP x`] DIV_MULT_LEM));
-
-val MOD_2EXP_LEM = Q.store_thm("MOD_2EXP_LEM",
-  `!n x. n MOD 2 EXP x = n - n DIV 2 EXP x * 2 EXP x`,
-  REPEAT STRIP_TAC
-    THEN ASSUME_TAC (Q.SPECL [`x`,`n`] DIV_MULT_LESS_EQ)
-    THEN RW_TAC std_ss [GSYM ADD_EQ_SUB]
-    THEN PROVE_TAC [ZERO_LT_TWOEXP,ADD_COMM,DIVISION]
-);
- 
-val DIV_MULT_LEM2 = prove(
-  `!a b p. a DIV 2 EXP (b + p) * 2 EXP (p + b) <= a DIV 2 EXP b * 2 EXP b`,
-  REPEAT STRIP_TAC
-    THEN ASSUME_TAC (SIMP_RULE std_ss [ZERO_LT_TWOEXP] 
-                      (SPECL [`a DIV 2 EXP b`,`2 EXP p`] DIV_MULT_LEM))
-    THEN ASM_SIMP_TAC std_ss [EXP_ADD,MULT_ASSOC,GSYM DIV_DIV_DIV_MULT,
-                              ZERO_LT_TWOEXP,LESS_MONO_MULT]
-);
- 
-val MOD_EXP_ADD = prove(
-  `!a b p. a MOD 2 EXP (b + p) 
-               = 
-           a MOD 2 EXP b + (a DIV 2 EXP b) MOD 2 EXP p * 2 EXP b`,
- REPEAT STRIP_TAC
-  THEN SIMP_TAC std_ss [MOD_2EXP_LEM,RIGHT_SUB_DISTRIB,DIV_DIV_DIV_MULT,
-                        ZERO_LT_TWOEXP,GSYM MULT_ASSOC,GSYM EXP_ADD]
-  THEN ASSUME_TAC (GSYM (
-        SPECL [`a DIV 2 EXP (b + p) * 2 EXP (p + b)`,
-               `a DIV 2 EXP b * 2 EXP b`] LESS_EQ_ADD_SUB))
-  THEN ASM_SIMP_TAC std_ss [DIV_MULT_LEM2,DIV_MULT_LEM,ZERO_LT_TWOEXP,SUB_ADD]
-  THEN PROVE_TAC [ADD_COMM]);
- 
-val DIV_MOD_MOD_DIV = prove(
-  `!a b p. (a DIV 2 EXP b) MOD 2 EXP p = a MOD 2 EXP (b + p) DIV 2 EXP b`,
-  REPEAT STRIP_TAC
-    THEN SIMP_TAC std_ss [MOD_EXP_ADD]
-    THEN ONCE_REWRITE_TAC [ADD_COMM]
-    THEN SIMP_TAC arith_ss [ADD_DIV_ADD_DIV,ZERO_LT_TWOEXP,LESS_DIV_EQ_ZERO,
-                 SIMP_RULE std_ss [ZERO_LT_TWOEXP] (SPEC `2 EXP b` DIVISION)]
-);
-
- 
-val DIV_MOD_MOD_DIV2 = prove(
-  `!a b c. (a DIV 2 EXP b) MOD 2 EXP (c - b) = (a MOD 2 EXP c) DIV 2 EXP b`,
-  REPEAT STRIP_TAC
-    THEN Cases_on `c <= b`
-    THENL [
-       `c - b = 0` by PROVE_TAC [SUB_EQ_0]
-          THEN RW_TAC arith_ss [REDUCE_RULE MOD_ONE]
-          THEN ASSUME_TAC (SPEC `a` 
-              (SIMP_RULE std_ss [ZERO_LT_TWOEXP] (SPEC `2 EXP c` DIVISION)))
-          THEN FULL_SIMP_TAC std_ss []
-          THEN IMP_RES_TAC LESS_EQUAL_ADD
-          THEN POP_ASSUM (fn th => REWRITE_TAC [th])
-          THEN ASSUME_TAC (GSYM (SIMP_RULE std_ss [ZERO_LT_TWOEXP]
-                           (SPECL [`2 EXP c`,`2 EXP p`] DIV_DIV_DIV_MULT)))
-          THEN ASM_SIMP_TAC std_ss 
-                   [EXP_ADD,LESS_DIV_EQ_ZERO,ZERO_DIV,ZERO_LT_TWOEXP],
-       RULE_ASSUM_TAC (REWRITE_RULE [NOT_LESS_EQUAL])
-          THEN IMP_RES_TAC LESS_ADD
-          THEN POP_ASSUM (fn th => REWRITE_TAC [SYM th])
-          THEN SIMP_TAC arith_ss [DIV_MOD_MOD_DIV]
-    ]
-);
-
-val BITS2_THM = store_thm("BITS2_THM",
-  `!h l n. BITS h l n = (n MOD 2 EXP SUC h) DIV 2 EXP l`,
-  RW_TAC std_ss [BITS_THM,DIV_MOD_MOD_DIV2]
-);
-
-val BITS_COMP_LEM = prove(
-  `!h1 l1 h2 l2 n. 
-      h2 + l1 <= h1 ==> 
-       (((n DIV 2 EXP l1) MOD 2 EXP (h1 - l1) DIV 2 EXP l2) MOD 2 EXP (h2-l2)
-         =
-       (n DIV 2 EXP (l2 + l1)) MOD 2 EXP ((h2 + l1) - (l2 + l1)))`,
-  REPEAT STRIP_TAC
-    THEN REWRITE_TAC [SPECL 
-          [`(n DIV 2 EXP l1) MOD 2 EXP (h1 - l1)`,`l2`,`h2`] DIV_MOD_MOD_DIV2]
-    THEN IMP_RES_TAC LESS_EQUAL_ADD
-    THEN POP_ASSUM (fn th => 
-           SIMP_TAC arith_ss [EXP_ADD,MOD_MULT_MOD,ZERO_LT_TWOEXP,th])
-    THEN REWRITE_TAC [SPECL [`n`,`l1`,`p`] DIV_MOD_MOD_DIV]
-    THEN SIMP_TAC arith_ss [DIV_DIV_DIV_MULT,ZERO_LT_TWOEXP,GSYM EXP_ADD]
-    THEN REWRITE_TAC [SIMP_RULE arith_ss [] 
-                       (SPECL [`n`,`l1 + l2`,`h2 + l1`] DIV_MOD_MOD_DIV2)]
-);
-
-val BITS_COMP_THM = store_thm("BITS_COMP_THM",
-  `!h1 l1 h2 l2 n. h2 + l1 <= h1 
-                    ==> (BITS h2 l2 (BITS h1 l1 n) = BITS (h2+l1) (l2+l1) n)`,
-  REPEAT STRIP_TAC
-    THEN IMP_RES_TAC LESS_EQ_MONO
-    THEN FULL_SIMP_TAC std_ss [BITS_THM,GSYM ADD_CLAUSES,BITS_COMP_LEM]
-);
-
-val BITS_DIV_THM = store_thm("BITS_DIV_THM",
-  `!h l x n. (BITS h l x) DIV 2 EXP n = BITS h (l + n) x`,
-  RW_TAC std_ss [BITS2_THM,EXP_ADD,ZERO_LT_TWOEXP,DIV_DIV_DIV_MULT]
-);
-
-val BITS_LT_HIGH = store_thm("BITS_LT_HIGH",
-  `!h l n. n < 2 EXP SUC h ==> (BITS h l n = n DIV 2 EXP l)`,
-  RW_TAC std_ss [BITS2_THM,LESS_MOD]
-);
-
-(* -------------------------------------------------------- *)
-
-val MOD2_EQ_0 = prove(
-  `!q. (q * 2) MOD 2 = 0`,
-  RW_TAC arith_ss [MOD_EQ_0]
-);
- 
-val ONE_TWO_LEM = prove(
-  `!n. (n MOD 2 = 0) \/ (n MOD 2 = 1)`,
-  `!n. n < 2 ==> ((n = 0) \/ (n = 1))` by DECIDE_TAC
-    THEN RW_TAC arith_ss [DIVISION]
-);
- 
-val NOT_MOD2_LEM = store_thm("NOT_MOD2_LEM",
-  `!n. ~(n MOD 2 = 0) = (n MOD 2 = 1)`,
-  STRIP_TAC THEN EQ_TAC
-    THENL [PROVE_TAC [ONE_TWO_LEM],DECIDE_TAC]
-);
-
-val EVEN_MOD2_LEM = store_thm("EVEN_MOD2_LEM",
-  `!n. EVEN n = ((n MOD 2) = 0)`,
-  RW_TAC std_ss [ONCE_REWRITE_RULE [MULT_COMM] EVEN_EXISTS]
-    THEN EQ_TAC THEN STRIP_TAC
-    THENL [
-      ASM_REWRITE_TAC [MOD2_EQ_0],
-      EXISTS_TAC `n DIV 2`
-        THEN `0 < 2n` by DECIDE_TAC
-        THEN IMP_RES_TAC DIVISION
-        THEN POP_ASSUM (K ALL_TAC)
-        THEN POP_ASSUM (fn th => ASSUME_TAC (SPEC `n` th))
-        THEN RW_TAC arith_ss []
-    ]
-);
- 
-val ODD_MOD2_LEM = store_thm("ODD_MOD2_LEM",
- `!n. ODD n = ((n MOD 2) = 1)`,
- STRIP_TAC THEN REWRITE_TAC [ODD_EVEN,EVEN_MOD2_LEM,NOT_MOD2_LEM]
-);
-
-(* -------------------------------------------------------- *)
-
+val MOD1 = REDUCE_RULE MOD_ONE;
 val DIV1 = save_thm("DIV1",REDUCE_RULE DIV_ONE);
 
-val LSB_ODD = store_thm("LSB_ODD",
-  `LSB = ODD`,
-  ONCE_REWRITE_TAC [FUN_EQ_THM]
-    THEN SIMP_TAC arith_ss [ODD_MOD2_LEM,LSB_def,BIT_def,BITS2_THM,EXP,DIV1]
+val SUC_SUB = save_thm("SUC_SUB",SIMP_CONV arithr_ss [ADD1] ``SUC a - a``);
+
+(* |- !n r. r < n ==> ((n + r) DIV n = 1) *)
+val DIV_MULT_1 = save_thm("DIV_MULT_1",
+  (GEN_ALL o SIMP_RULE arith_ss [] o INST [`q` |-> `1`] o SPEC_ALL
+           o CONV_RULE (ONCE_DEPTH_CONV RIGHT_IMP_FORALL_CONV)) DIV_MULT
 );
 
-(* -------------------------------------------------------- *)
-
-val DIV_MULT_THM = store_thm("DIV_MULT_THM",
-  `!x n. n DIV 2 EXP x * 2 EXP x = n - n MOD 2 EXP x`,
-  RW_TAC arith_ss [DIV_MULT_LESS_EQ,MOD_2EXP_LEM,SUB_SUB]
-);
- 
-val DIV_MULT_THM2 = save_thm("DIV_MULT_THM2",
-  ONCE_REWRITE_RULE [MULT_COMM] (REWRITE_RULE [EXP_1] (SPEC `1` DIV_MULT_THM))
+(* |- !m. ~(m = 0) ==> ?p. m = SUC p *)
+val NOT_ZERO_ADD1 = save_thm("NOT_ZERO_ADD1",
+  (GEN_ALL o REWRITE_RULE [GSYM NOT_ZERO_LT_ZERO,GSYM ADD1,ADD] o SPECL [`m`,`0`]) LESS_ADD_1
 );
 
-val MULT_INCREASES2 = 
- ONCE_REWRITE_RULE [MULT_COMM] (REWRITE_RULE [GSYM LESS_EQ] MULT_INCREASES);
+val ZERO_LT_TWOEXP = save_thm("ZERO_LT_TWOEXP",
+  GEN_ALL (REDUCE_RULE (SPECL [`n`,`1`] ZERO_LESS_EXP))
+);
+
+val th = (SPEC_ALL o REWRITE_RULE [ZERO_LT_TWOEXP] o SPEC `2 EXP n`) DIVISION;
+
+(* |- !n k. k MOD 2 EXP n < 2 EXP n *)
+val MOD_2EXP_LT = save_thm("MOD_2EXP_LT",
+  (GEN_ALL o CONJUNCT2) th
+);
+
+(* |- !n k. k = k DIV 2 EXP n * 2 EXP n + k MOD 2 EXP n *)
+val TWOEXP_DIVISION = save_thm("TWOEXP_DIVISION",
+  (GEN_ALL o CONJUNCT1) th
+);
+
+val MULT_INCREASES2 = ONCE_REWRITE_RULE [MULT_COMM] (REWRITE_RULE [GSYM LESS_EQ] MULT_INCREASES);
 
 val ONE_LT_TWOEXP_SUCN = prove(
   `!n. 1 < 2 EXP n * 2`,
-  Induct_on `n` THEN RW_TAC arith_ss [EXP,MULT_INCREASES2]
+  Induct_on `n` THEN A_RW_TAC [EXP,MULT_INCREASES2]
 );
  
 val TWOEXP_MONO = store_thm("TWOEXP_MONO",
   `!a b. a < b ==> 2 EXP a < 2 EXP b`,
   REPEAT STRIP_TAC
     THEN IMP_RES_TAC LESS_ADD_1
-    THEN ASM_SIMP_TAC arith_ss 
-           [EXP_ADD,MULT_INCREASES2,ONE_LT_TWOEXP_SUCN,ZERO_LT_TWOEXP]
+    THEN ASM_R_SIMP_TAC [EXP_ADD,MULT_INCREASES2,ONE_LT_TWOEXP_SUCN,ZERO_LT_TWOEXP]
 );
  
 val TWOEXP_MONO2 = store_thm("TWOEXP_MONO2",
   `!a b. a <= b ==> 2 EXP a <= 2 EXP b`,
   REPEAT STRIP_TAC
     THEN Cases_on `b = a`
-    THEN FULL_SIMP_TAC arith_ss [GSYM NOT_LESS]
+    THEN A_FULL_SIMP_TAC [GSYM NOT_LESS]
     THEN IMP_RES_TAC LESS_CASES_IMP
-    THEN RW_TAC std_ss [TWOEXP_MONO,NOT_LESS,LESS_IMP_LESS_OR_EQ]
+    THEN B_RW_TAC [TWOEXP_MONO,NOT_LESS,LESS_IMP_LESS_OR_EQ]
 );
 
-val LESS_EXP_MULT = store_thm("LESS_EXP_MULT",
-  `!a b. a < b ==> ?p. 2 EXP b = p * 2 EXP a`,
-  REPEAT STRIP_TAC
-    THEN IMP_RES_TAC LESS_ADD
-    THEN RULE_ASSUM_TAC (ONCE_REWRITE_RULE [SIMP_RULE arith_ss [] (SPEC `2` (GSYM EXP_INJECTIVE))])
-    THEN EXISTS_TAC `2 EXP p`
-    THEN FULL_SIMP_TAC arith_ss [EXP_ADD]
+val EXP_SUB_LESS_EQ = store_thm("EXP_SUB_LESS_EQ",
+  `!a b. 2 EXP (a - b) <= 2 EXP a`,
+  B_RW_TAC [SUB_LESS_EQ,TWOEXP_MONO2]
+);
+
+(* -------------------------------------------------------- *)
+
+val BITS_THM = save_thm("BITS_THM",
+  REWRITE_RULE [DIV_2EXP_def,MOD_2EXP_def] BITS_def
+);
+
+val BITSLT_THM = store_thm("BITSLT_THM",
+  `!h l n. BITS h l n < 2 EXP (SUC h-l)`,
+  B_RW_TAC [BITS_THM,ZERO_LT_TWOEXP,DIVISION]
+);
+
+val DIV_MULT_LEM = store_thm("DIV_MULT_LEM",
+  `!m n. 0 < n ==> m DIV n * n <= m`,
+  A_RW_TAC [LESS_EQ_EXISTS]
+    THEN EXISTS_TAC `m MOD n`
+    THEN A_RW_TAC [GSYM DIVISION]
 );
  
+(* |- !x n. n DIV 2 EXP x * 2 EXP x <= n *)
+val DIV_MULT_LESS_EQ = GEN_ALL (SIMP_RULE bool_ss [ZERO_LT_TWOEXP] (SPECL [`n`,`2 EXP x`] DIV_MULT_LEM));
+
+val MOD_2EXP_LEM = store_thm("MOD_2EXP_LEM",
+  `!n x. n MOD 2 EXP x = n - n DIV 2 EXP x * 2 EXP x`,
+  A_RW_TAC [DIV_MULT_LESS_EQ,GSYM ADD_EQ_SUB,ZERO_LT_TWOEXP,GSYM DIVISION]
+);
+ 
+val DIV_MULT_LEM2 = prove(
+  `!a b p. a DIV 2 EXP (b + p) * 2 EXP (p + b) <= a DIV 2 EXP b * 2 EXP b`,
+  B_RW_TAC [SPECL [`a DIV 2 EXP b`,`2 EXP p`] DIV_MULT_LEM,
+            EXP_ADD,MULT_ASSOC,GSYM DIV_DIV_DIV_MULT,ZERO_LT_TWOEXP,LESS_MONO_MULT]
+);
+ 
+val MOD_EXP_ADD = prove(
+  `!a b p. a MOD 2 EXP (b + p) = a MOD 2 EXP b + (a DIV 2 EXP b) MOD 2 EXP p * 2 EXP b`,
+  REPEAT STRIP_TAC
+    THEN B_SIMP_TAC [MOD_2EXP_LEM,RIGHT_SUB_DISTRIB,DIV_DIV_DIV_MULT,
+                     ZERO_LT_TWOEXP,GSYM MULT_ASSOC,GSYM EXP_ADD]
+    THEN ASSUME_TAC (
+           (GSYM o SPECL [`a DIV 2 EXP (b + p) * 2 EXP (p + b)`,`a DIV 2 EXP b * 2 EXP b`]) LESS_EQ_ADD_SUB)
+    THEN ASM_A_SIMP_TAC [DIV_MULT_LEM2,DIV_MULT_LEM,ZERO_LT_TWOEXP,SUB_ADD]
+);
+ 
+val DIV_MOD_MOD_DIV = prove(
+  `!a b p. (a DIV 2 EXP b) MOD 2 EXP p = a MOD 2 EXP (b + p) DIV 2 EXP b`,
+  A_RW_TAC [MOD_EXP_ADD,ADD_DIV_ADD_DIV,ZERO_LT_TWOEXP,LESS_DIV_EQ_ZERO,DIVISION]
+);
+ 
+val DIV_MOD_MOD_DIV2 = prove(
+  `!a b c. (a DIV 2 EXP b) MOD 2 EXP (c - b) = (a MOD 2 EXP c) DIV 2 EXP b`,
+  REPEAT STRIP_TAC
+    THEN Cases_on `c <= b`
+    THENL [
+       POP_ASSUM (fn th => REWRITE_TAC [REWRITE_RULE [GSYM SUB_EQ_0] th,EXP,MOD1]
+                             THEN ASSUME_TAC (MATCH_MP TWOEXP_MONO2 th))
+         THEN ASSUME_TAC (SPECL [`c`,`a`] MOD_2EXP_LT)
+         THEN IMP_RES_TAC LESS_LESS_EQ_TRANS
+         THEN ASM_B_SIMP_TAC [LESS_DIV_EQ_ZERO],
+       RULE_ASSUM_TAC (REWRITE_RULE [NOT_LESS_EQUAL])
+          THEN IMP_RES_TAC LESS_ADD
+          THEN POP_ASSUM (fn th => A_SIMP_TAC [SYM th,DIV_MOD_MOD_DIV])
+    ]
+);
+
+val BITS2_THM = store_thm("BITS2_THM",
+  `!h l n. BITS h l n = (n MOD 2 EXP SUC h) DIV 2 EXP l`,
+  B_RW_TAC [BITS_THM,DIV_MOD_MOD_DIV2]
+);
+
+val BITS_COMP_LEM = prove(
+  `!h1 l1 h2 l2 n. h2 + l1 <= h1 ==>
+    (((n DIV 2 EXP l1) MOD 2 EXP (h1 - l1) DIV 2 EXP l2) MOD 2 EXP (h2 - l2) =
+      (n DIV 2 EXP (l2 + l1)) MOD 2 EXP ((h2 + l1) - (l2 + l1)))`,
+  REPEAT STRIP_TAC
+    THEN REWRITE_TAC [SPECL [`(n DIV 2 EXP l1) MOD 2 EXP (h1 - l1)`,`l2`,`h2`] DIV_MOD_MOD_DIV2]
+    THEN IMP_RES_TAC LESS_EQUAL_ADD
+    THEN POP_ASSUM (fn th => A_SIMP_TAC [EXP_ADD,MOD_MULT_MOD,ZERO_LT_TWOEXP,th])
+    THEN REWRITE_TAC [DIV_MOD_MOD_DIV]
+    THEN A_SIMP_TAC [DIV_DIV_DIV_MULT,ZERO_LT_TWOEXP,GSYM EXP_ADD]
+    THEN REWRITE_TAC [SIMP_RULE arith_ss [] (SPECL [`n`,`l1 + l2`,`h2 + l1`] DIV_MOD_MOD_DIV2)]
+);
+
+val BITS_COMP_THM = store_thm("BITS_COMP_THM",
+  `!h1 l1 h2 l2 n. h2 + l1 <= h1 ==> (BITS h2 l2 (BITS h1 l1 n) = BITS (h2+l1) (l2+l1) n)`,
+  REPEAT STRIP_TAC
+    THEN IMP_RES_TAC LESS_EQ_MONO
+    THEN B_FULL_SIMP_TAC [BITS_THM,GSYM ADD_CLAUSES,BITS_COMP_LEM]
+);
+
+val BITS_DIV_THM = store_thm("BITS_DIV_THM",
+  `!h l x n. (BITS h l x) DIV 2 EXP n = BITS h (l + n) x`,
+  B_RW_TAC [BITS2_THM,EXP_ADD,ZERO_LT_TWOEXP,DIV_DIV_DIV_MULT]
+);
+
+val BITS_LT_HIGH = store_thm("BITS_LT_HIGH",
+  `!h l n. n < 2 EXP SUC h ==> (BITS h l n = n DIV 2 EXP l)`,
+  B_RW_TAC [BITS2_THM,LESS_MOD]
+);
+
+(* -------------------------------------------------------- *)
+
+val BITS_ZERO = store_thm("BITS_ZERO",
+  `!h l n. h < l ==> (BITS h l n = 0)`,
+  REPEAT STRIP_TAC
+    THEN IMP_RES_TAC LESS_ADD_1
+    THEN POP_ASSUM (fn th => REWRITE_TAC [th])
+    THEN ASSUME_TAC ((REWRITE_RULE [EXP,SUB,SUB_EQUAL_0] o ONCE_REWRITE_RULE [SUB_PLUS] o
+                        REWRITE_RULE [ADD1] o SPECL [`h`,`h + 1 + p`,`n`]) BITSLT_THM)
+    THEN A_FULL_SIMP_TAC []
+);
+ 
+val BITS_ZERO2 = store_thm("BITS_ZERO2",
+  `!h l. BITS h l 0 = 0`,
+  B_RW_TAC [BITS2_THM,ZERO_MOD,ZERO_DIV,ZERO_LT_TWOEXP]
+);
+
+(* |- !h n. BITS h 0 n = n MOD 2 EXP SUC h *)
+val BITS_ZERO3 = save_thm("BITS_ZERO3",
+  (GEN_ALL o SIMP_RULE bool_ss [CONJUNCT1 EXP,DIV1] o SPECL [`h`,`0`]) BITS2_THM
+);
+
+(* -------------------------------------------------------- *)
+
+val BITS_COMP_THM2 = store_thm("BITS_COMP_THM2",
+  `!h1 l1 h2 l2 n. BITS h2 l2 (BITS h1 l1 n) = BITS (MIN h1 (h2 + l1)) (l2 + l1) n`,
+  B_RW_TAC [MIN_DEF,REWRITE_RULE [GSYM NOT_LESS] BITS_COMP_THM]
+    THEN Cases_on `h2 = 0`
+    THENL [
+      A_FULL_SIMP_TAC [BITS_ZERO,BITS_ZERO2],
+      RULE_ASSUM_TAC (REWRITE_RULE [NOT_ZERO_LT_ZERO])
+        THEN Cases_on `h1 < l1`
+        THENL [
+          A_FULL_SIMP_TAC [BITS_ZERO,BITS_ZERO2],
+          RULE_ASSUM_TAC (ONCE_REWRITE_RULE [ADD_COMM])
+            THEN IMP_RES_TAC SUB_RIGHT_LESS
+            THEN POP_ASSUM (fn th => ASSUME_TAC
+                   (MATCH_MP TWOEXP_MONO (ONCE_REWRITE_RULE [GSYM LESS_MONO_EQ] th)))
+            THEN ASSUME_TAC (SPECL [`h1`,`l1`,`n`] BITSLT_THM)
+            THEN Cases_on `h1 = l1`
+            THENL [
+               A_FULL_SIMP_TAC [SYM ONE,SUC_SUB]
+                 THEN `BITS h1 l1 n < 2 EXP SUC h2` by IMP_RES_TAC LESS_TRANS
+                 THEN ASM_A_SIMP_TAC [BITS_LT_HIGH,BITS_DIV_THM],
+               `~(h1 <= l1)` by DECIDE_TAC
+                 THEN POP_ASSUM (fn th => RULE_ASSUM_TAC (SIMP_RULE bool_ss [th,SUB_LEFT_SUC]))
+                 THEN `BITS h1 l1 n < 2 EXP SUC h2` by IMP_RES_TAC LESS_TRANS
+                 THEN ASM_A_SIMP_TAC [BITS_LT_HIGH,BITS_DIV_THM]
+            ]
+        ]
+    ]
+);
+
+(* -------------------------------------------------------- *)
+
+val MOD2_EQ_0 = prove(
+  `!q. (q * 2) MOD 2 = 0`,
+  A_RW_TAC [MOD_EQ_0]
+);
+ 
+val ONE_TWO_LEM = prove(
+  `!n. (n MOD 2 = 0) \/ (n MOD 2 = 1)`,
+  `!n. n < 2 ==> ((n = 0) \/ (n = 1))` by DECIDE_TAC
+    THEN A_RW_TAC [DIVISION]
+);
+ 
+val NOT_MOD2_LEM = store_thm("NOT_MOD2_LEM",
+  `!n. ~(n MOD 2 = 0) = (n MOD 2 = 1)`,
+  STRIP_TAC THEN ASSUME_TAC (SPEC `n` ONE_TWO_LEM) THEN EQ_TAC THEN A_RW_TAC []
+);
+
+val NOT_MOD2_LEM2 = store_thm("NOT_MOD2_LEM2",
+  `!n a. ~(n MOD 2 = 1) = (n MOD 2 = 0)`,
+  B_RW_TAC [GSYM NOT_MOD2_LEM]
+);
+ 
+val EVEN_MOD2_LEM = store_thm("EVEN_MOD2_LEM",
+  `!n. EVEN n = ((n MOD 2) = 0)`,
+  B_RW_TAC [ONCE_REWRITE_RULE [MULT_COMM] EVEN_EXISTS]
+    THEN EQ_TAC THEN STRIP_TAC
+    THENL [
+      ASM_REWRITE_TAC [MOD2_EQ_0],
+      EXISTS_TAC `n DIV 2`
+        THEN ASSUME_TAC ((SPEC `n` o REWRITE_RULE [EXP_1] o SPEC `1`) TWOEXP_DIVISION)
+        THEN A_RW_TAC []
+    ]
+);
+ 
+val ODD_MOD2_LEM = store_thm("ODD_MOD2_LEM",
+ `!n. ODD n = ((n MOD 2) = 1)`,
+  STRIP_TAC THEN REWRITE_TAC [ODD_EVEN,EVEN_MOD2_LEM,NOT_MOD2_LEM]
+);
+
+(* -------------------------------------------------------- *)
+
+val LSB_ODD = store_thm("LSB_ODD",
+  `LSB = ODD`,
+  ONCE_REWRITE_TAC [FUN_EQ_THM]
+    THEN A_SIMP_TAC [ODD_MOD2_LEM,LSB_def,BIT_def,BITS2_THM,EXP,DIV1]
+);
+
+(* -------------------------------------------------------- *)
+
+val DIV_MULT_THM = store_thm("DIV_MULT_THM",
+  `!x n. n DIV 2 EXP x * 2 EXP x = n - n MOD 2 EXP x`,
+  A_RW_TAC [DIV_MULT_LESS_EQ,MOD_2EXP_LEM,SUB_SUB]
+);
+ 
+val DIV_MULT_THM2 = save_thm("DIV_MULT_THM2",
+  ONCE_REWRITE_RULE [MULT_COMM] (REWRITE_RULE [EXP_1] (SPEC `1` DIV_MULT_THM))
+);
+
 val LESS_EQ_EXP_MULT = store_thm("LESS_EQ_EXP_MULT",
   `!a b. a <= b ==> ?p. 2 EXP b = p * 2 EXP a`,
   REPEAT STRIP_TAC
@@ -270,31 +319,31 @@ val LESS_EQ_EXP_MULT = store_thm("LESS_EQ_EXP_MULT",
     THEN FULL_SIMP_TAC arith_ss [EXP_ADD,MULT_COMM]
 );
 
+val LESS_EXP_MULT = (EQT_ELIM o SIMP_CONV bool_ss [LESS_IMP_LESS_OR_EQ,LESS_EQ_EXP_MULT])
+                      ``!a b. a < b ==> ?p. 2 EXP b = p * 2 EXP a``;
+ 
 (* -------------------------------------------------------- *)
 
 val SLICE_LEM1 = store_thm("SLICE_LEM1",
-  `!a x y. a DIV 2 EXP (x+y) * 2 EXP (x+y) =
+  `!a x y. a DIV 2 EXP (x + y) * 2 EXP (x + y) =
        a DIV 2 EXP x * 2 EXP x - (a DIV 2 EXP x) MOD 2 EXP y * 2 EXP x`,
   REPEAT STRIP_TAC
-    THEN SIMP_TAC std_ss [EXP_ADD]
+    THEN REWRITE_TAC [EXP_ADD]
     THEN SUBST_OCCS_TAC [([2],SPECL [`2 EXP x`,`2 EXP y`] MULT_COMM)]
-    THEN SIMP_TAC std_ss [ZERO_LT_TWOEXP,GSYM DIV_DIV_DIV_MULT,MULT_ASSOC,
-             SPECL [`y`,`a DIV 2 EXP x`] DIV_MULT_THM,RIGHT_SUB_DISTRIB]
+    THEN B_SIMP_TAC [ZERO_LT_TWOEXP,GSYM DIV_DIV_DIV_MULT,MULT_ASSOC,
+                     SPECL [`y`,`a DIV 2 EXP x`] DIV_MULT_THM,RIGHT_SUB_DISTRIB]
 );
 
 val SLICE_LEM2 = store_thm("SLICE_LEM2",
-  `!a x y. n MOD 2 EXP (x+y) 
-            = 
-           n MOD 2 EXP x + (n DIV 2 EXP x) MOD 2 EXP y * 2 EXP x`,
+  `!a x y. n MOD 2 EXP (x + y) = n MOD 2 EXP x + (n DIV 2 EXP x) MOD 2 EXP y * 2 EXP x`,
   REPEAT STRIP_TAC
-    THEN SIMP_TAC std_ss [DIV_MULT_LESS_EQ,MOD_2EXP_LEM,SLICE_LEM1,
-                          RIGHT_SUB_DISTRIB,SUB_SUB,SUB_LESS_EQ]
+    THEN B_SIMP_TAC [DIV_MULT_LESS_EQ,MOD_2EXP_LEM,SLICE_LEM1,RIGHT_SUB_DISTRIB,SUB_SUB,SUB_LESS_EQ]
     THEN Cases_on `n = n DIV 2 EXP x * 2 EXP x`
     THENL [
-       POP_ASSUM (fn th => SIMP_TAC arith_ss [SYM th]),
+       POP_ASSUM (fn th => A_SIMP_TAC [SYM th]),
        ASSUME_TAC (REWRITE_RULE [GSYM NOT_LESS] DIV_MULT_LESS_EQ)
          THEN IMP_RES_TAC LESS_CASES_IMP
-         THEN RW_TAC std_ss [SUB_RIGHT_ADD]
+         THEN B_RW_TAC [SUB_RIGHT_ADD]
          THEN PROVE_TAC [GSYM NOT_LESS_EQUAL]
     ]
 );
@@ -305,7 +354,7 @@ val SLICE_LEM3 = store_thm("SLICE_LEM3",
     THEN IMP_RES_TAC LESS_ADD_1
     THEN POP_ASSUM (fn th => REWRITE_TAC [th])
     THEN REWRITE_TAC [GSYM ADD1,GSYM ADD_SUC,GSYM (CONJUNCT2 ADD)]
-    THEN RW_TAC arith_ss [SLICE_LEM2]
+    THEN A_SIMP_TAC [SLICE_LEM2]
 );
 
 val SLICE_THM = store_thm("SLICE_THM",
@@ -318,63 +367,87 @@ val SLICE_THM = store_thm("SLICE_THM",
         THEN POP_ASSUM (fn th => ASSUME_TAC (SPEC `n` th))
         THEN IMP_RES_TAC LESS_OR
         THEN IMP_RES_TAC SUB_EQ_0
-        THEN ASM_SIMP_TAC arith_ss [EXP,REDUCE_RULE MOD_ONE,MULT_CLAUSES],
+        THEN ASM_SIMP_TAC arith_ss [EXP,MOD1,MULT_CLAUSES],
       REWRITE_TAC [DIV_MOD_MOD_DIV2]
         THEN RULE_ASSUM_TAC (REWRITE_RULE [NOT_LESS])
-        THEN SUBST_OCCS_TAC [([1],CONJUNCT1 (SPEC `n MOD 2 EXP SUC h` (
-                SIMP_RULE std_ss [ZERO_LT_TWOEXP] (SPEC `2 EXP l` DIVISION))))]
+        THEN SUBST_OCCS_TAC [([1],SPECL [`l`,`n MOD 2 EXP SUC h`] TWOEXP_DIVISION)]
         THEN IMP_RES_TAC LESS_EQUAL_ADD
         THEN POP_ASSUM (fn th => SUBST_OCCS_TAC [([2],th)])
-        THEN SIMP_TAC std_ss 
-               [ADD_SUC,ADD_SUB,MOD_MULT_MOD,ZERO_LT_TWOEXP,EXP_ADD]
+        THEN B_SIMP_TAC [ADD_SUC,ADD_SUB,MOD_MULT_MOD,ZERO_LT_TWOEXP,EXP_ADD]
     ]
 );
 
 val SLICELT_THM = store_thm("SLICELT_THM",
   `!h l n. SLICE h l n < 2 EXP SUC h`,
   REPEAT STRIP_TAC
-    THEN ASSUME_TAC 
-           (CONJUNCT2 
-              (SPEC `n` 
-                (SIMP_RULE std_ss [ZERO_LT_TWOEXP] 
-                   (SPEC `2 EXP SUC h` DIVISION))))
-    THEN RW_TAC arith_ss 
-          [SLICE_def,MOD_2EXP_def,ZERO_LT_TWOEXP,SUB_RIGHT_LESS]);
+    THEN ASSUME_TAC (SPECL [`SUC h`,`n`] MOD_2EXP_LT)
+    THEN R_RW_TAC [SLICE_def,MOD_2EXP_def,ZERO_LT_TWOEXP,SUB_RIGHT_LESS]
+);
  
 val BITS_SLICE_THM = store_thm("BITS_SLICE_THM",
   `!h l n. BITS h l (SLICE h l n) = BITS h l n`,
-  RW_TAC std_ss [SLICELT_THM,BITS_LT_HIGH,ZERO_LT_TWOEXP,SLICE_THM,MULT_DIV]
+  B_RW_TAC [SLICELT_THM,BITS_LT_HIGH,ZERO_LT_TWOEXP,SLICE_THM,MULT_DIV]
 );
 
 val MOD_2EXP_MONO = store_thm("MOD_2EXP_MONO",
   `!n h l. l <= h ==> n MOD 2 EXP l <= n MOD 2 EXP SUC h`,
   REPEAT STRIP_TAC
     THEN IMP_RES_TAC LESS_EQ_EXISTS
-    THEN POP_ASSUM (fn th => REWRITE_TAC [th])
-    THEN `SUC (l + p) = l + SUC p` by DECIDE_TAC
-    THEN RW_TAC arith_ss [SLICE_LEM2]
+    THEN ASM_A_SIMP_TAC [SUC_ADD_SYM,SLICE_LEM2]
 );
 
 val SLICE_COMP_THM = store_thm("SLICE_COMP_THM",
-  `!h m l n. (SUC m) <= h /\ l <= m 
-              ==> 
-             (SLICE h (SUC m) n + SLICE m l n = SLICE h l n)`,
-  RW_TAC std_ss 
-     [SLICE_def,MOD_2EXP_def,MOD_2EXP_MONO,GSYM LESS_EQ_ADD_SUB,SUB_ADD]
+  `!h m l n. (SUC m) <= h /\ l <= m ==> (SLICE h (SUC m) n + SLICE m l n = SLICE h l n)`,
+  B_RW_TAC [SLICE_def,MOD_2EXP_def,MOD_2EXP_MONO,GSYM LESS_EQ_ADD_SUB,SUB_ADD]
 );
 
 (* -------------------------------------------------------- *)
 
-val SUC_SUB = SIMP_CONV arith_ss [ADD1] ``SUC a - a``;
- 
+val ssd = SIMPSET {ac = [(SPEC_ALL MULT_ASSOC, SPEC_ALL MULT_COMM)],
+                congs = [], convs = [], dprocs = [], filter = NONE, rewrs = []};
+val arith2_ss = arith_ss++ssd;
+
+val lem  = prove(`!c a b. (a = b) ==> (a DIV c = b DIV c)`, A_RW_TAC []);
+val lem2 = prove(`!a b c. a * (b * c) = a * c * b`, SIMP_TAC arith2_ss []);
+
+val lem3 = prove(
+  `!a m n. n <= m ==> (a * 2 EXP m DIV 2 EXP n = a * 2 EXP (m - n))`,
+  REPEAT STRIP_TAC
+    THEN IMP_RES_TAC LESS_EQUAL_ADD
+    THEN ASM_SIMP_TAC arith_ss [EXP_ADD,MULT_DIV,ZERO_LT_TWOEXP,lem2]
+);
+
+(* |- !a m n. n < m ==> (a * 2 EXP m DIV 2 EXP n = a * 2 EXP (m - n)) *)
+val lem4 = EQT_ELIM (SIMP_CONV std_ss [LESS_IMP_LESS_OR_EQ,lem3]
+             ``!a m n. n < m ==> (a * 2 EXP m DIV 2 EXP n = a * 2 EXP (m - n))``);
+
+val BIT_COMP_THM3 = store_thm("BIT_COMP_THM3",
+  `!h m l n.  SUC m <= h /\ l <= m ==>
+         (BITS h (SUC m) n * 2 EXP (SUC m - l) + BITS m l n = BITS h l n)`,
+  REPEAT STRIP_TAC
+    THEN IMP_RES_TAC (REWRITE_RULE [SLICE_THM] SLICE_COMP_THM)
+    THEN POP_ASSUM (K ALL_TAC)
+    THEN POP_ASSUM (fn th => ASSUME_TAC (GEN `l'` (MATCH_MP (SPEC `2 EXP l` lem) (SPEC `n` th))))
+    THEN POP_ASSUM (fn th => ASSUME_TAC (ONCE_REWRITE_RULE [ADD_COMM] (SPEC `l` th)))
+    THEN `l < SUC m` by ASM_A_SIMP_TAC []
+    THEN A_FULL_SIMP_TAC [lem4,ADD_DIV_ADD_DIV,MULT_DIV,ZERO_LT_TWOEXP]
+);
+
+(* -------------------------------------------------------- *)
+
 val NOT_BIT = store_thm("NOT_BIT",
   `!n a. ~BIT n a = (BITS n n a = 0)`,
-  RW_TAC std_ss [BIT_def,BITS_THM,SUC_SUB,EXP_1,GSYM NOT_MOD2_LEM]
+  B_RW_TAC [BIT_def,BITS_THM,SUC_SUB,EXP_1,GSYM NOT_MOD2_LEM]
 );
  
 val NOT_BITS = store_thm("NOT_BITS",
   `!n a. ~(BITS n n a = 0) = (BITS n n a = 1)`,
-  RW_TAC std_ss [GSYM NOT_BIT,GSYM BIT_def]
+  B_RW_TAC [GSYM NOT_BIT,GSYM BIT_def]
+);
+ 
+val NOT_BITS2 = store_thm("NOT_BITS2",
+  `!n a. ~(BITS n n a = 1) = (BITS n n a = 0)`,
+  B_RW_TAC [GSYM NOT_BITS]
 );
  
 val BIT_SLICE = store_thm("BIT_SLICE",
@@ -382,72 +455,76 @@ val BIT_SLICE = store_thm("BIT_SLICE",
   REPEAT STRIP_TAC THEN EQ_TAC
     THENL [
       Cases_on `BIT n a`
-        THEN FULL_SIMP_TAC arith_ss [BIT_def,SLICE_THM]
-        THEN FULL_SIMP_TAC arith_ss [GSYM NOT_BITS],
+        THEN A_FULL_SIMP_TAC [BIT_def,SLICE_THM,NOT_BITS2],
       Cases_on `BITS n n a = 1`
         THEN Cases_on `BITS n n b = 1`
-        THEN FULL_SIMP_TAC arith_ss [BIT_def,SLICE_THM]
-        THEN FULL_SIMP_TAC arith_ss [GSYM NOT_BITS,MULT_CLAUSES,
-                                     REWRITE_RULE [GSYM NOT_ZERO_LT_ZERO] ZERO_LT_TWOEXP]
+        THEN A_FULL_SIMP_TAC [BIT_def,SLICE_THM,NOT_BITS2,MULT_CLAUSES,
+                              REWRITE_RULE [GSYM NOT_ZERO_LT_ZERO] ZERO_LT_TWOEXP]
     ]
 );
 
-val BITS_ZERO = store_thm("BITS_ZERO",
-  `!h l n. h < l ==> (BITS h l n = 0)`,
-  REPEAT STRIP_TAC
-    THEN IMP_RES_TAC LESS_ADD_1
-    THEN POP_ASSUM (fn th => REWRITE_TAC [th])
-    THEN ASSUME_TAC (REWRITE_RULE [EXP,SUB,SUB_EQUAL_0]
-                       (ONCE_REWRITE_RULE [SUB_PLUS]
-                          (REWRITE_RULE [ADD1] (SPECL [`h`,`h + 1 + p`,`n`] BITSLT_THM))))
-    THEN FULL_SIMP_TAC arith_ss []
+val BIT_SLICE_LEM = store_thm("BIT_SLICE_LEM",
+  `!y x n. SET (BIT x n) (x + y) = (SLICE x x n) * 2 EXP y`,
+  A_RW_TAC [SET_def,BIT_SLICE,SLICE_THM,BIT_def,EXP_ADD]
+    THEN B_FULL_SIMP_TAC [GSYM NOT_BITS]
 );
- 
+
+(* |- !x n. SET (BIT x n) x = SLICE x x n *)
+val BIT_SLICE_THM = save_thm("BIT_SLICE_THM",
+   SIMP_RULE arith_ss [EXP] (SPEC `0` BIT_SLICE_LEM)
+);
+
 val SUB_BITS = prove(
   `!h l a b. (BITS (SUC h) l a = BITS (SUC h) l b) ==> (BITS h l a = BITS h l b)`,
   REPEAT STRIP_TAC
     THEN Cases_on `h < l`
     THENL [
-      RW_TAC std_ss [BITS_ZERO],
+      B_RW_TAC [BITS_ZERO],
       RULE_ASSUM_TAC (REWRITE_RULE [NOT_LESS])
         THEN POP_ASSUM (fn th =>
-               ONCE_REWRITE_TAC [GSYM (SIMP_RULE arith_ss [th,SUB_ADD]
-               (SPECL [`SUC h`,`l`,`h-l`,`0`] BITS_COMP_THM))])
+               ONCE_REWRITE_TAC [(GSYM o SIMP_RULE arith_ss [th,SUB_ADD] o
+                                  SPECL [`SUC h`,`l`,`h - l`,`0`]) BITS_COMP_THM])
         THEN ASM_REWRITE_TAC []
     ]
+);
+ 
+val SET_DIV = store_thm("SET_DIV",
+  `!b m n. n < m ==> (SET b (m - n) = SET b m DIV 2 EXP n)`,
+  B_RW_TAC [SET_def,ZERO_DIV,ZERO_LT_TWOEXP,SIMP_RULE arith_ss [] (SPEC `1` lem4)]
+);
+
+val BITS_SUC = store_thm("BITS_SUC",
+  `!h l n.  l <= SUC h ==>
+         (SET (BIT (SUC h) n) (SUC h - l) + BITS h l n = BITS (SUC h) l n)`,
+  REPEAT STRIP_TAC
+    THEN Cases_on `l = SUC h`
+    THENL [
+      A_RW_TAC [EXP,BITS_ZERO,SET_def,BIT_def]
+        THEN B_FULL_SIMP_TAC [NOT_BITS2],
+      `l <= h` by ASM_A_SIMP_TAC []
+        THEN IMP_RES_TAC LESS_EQ_IMP_LESS_SUC
+        THEN ASM_A_SIMP_TAC [SET_DIV,BIT_SLICE_THM,SLICE_THM,lem4,SPECL [`SUC h`,`h`] BIT_COMP_THM3]
+    ]
+);
+
+val BITS_SUC_THM = store_thm("BITS_SUC_THM",
+  `!h l n. BITS (SUC h) l n = if SUC h < l
+                              then 0
+                              else SET (BIT (SUC h) n) (SUC h - l) + BITS h l n`,
+  A_RW_TAC [BITS_ZERO,BITS_SUC]
 );
 
 val DECEND_LEMMA = prove(
   `!P l y.  (!x. l <= x /\ x <= SUC y ==> P x) ==> (!x. l <= x /\ x <= y ==> P x)`,
-  RW_TAC arith_ss []
+  A_RW_TAC []
 );
  
-(* |- !m n. m < SUC n ==> m <= n *)
-val LESS_LEMMA3 = REWRITE_RULE [ONCE_REWRITE_RULE [DISJ_COMM] (GSYM LESS_OR_EQ)] LESS_LEMMA1;
-
-val BITS_SUC = prove(
-  `!h l a. BITS (SUC h) l a = if l = SUC h then
-                                BITS (SUC h) l (SLICE (SUC h) (SUC h) a)
-                              else
-                                BITS (SUC h) l (SLICE (SUC h) (SUC h) a + BITS h l a * 2 EXP l)`,
-  REPEAT STRIP_TAC
-    THEN Cases_on `SUC h < l`
-    THENL [
-      RW_TAC std_ss [BITS_ZERO],
-      RULE_ASSUM_TAC (REWRITE_RULE [NOT_LESS])
-        THEN RW_TAC arith_ss [GSYM SLICE_THM,BITS_SLICE_THM]
-        THEN `l < SUC h` by ASM_SIMP_TAC arith_ss []
-        THEN IMP_RES_TAC LESS_LEMMA3
-        THEN ASM_SIMP_TAC std_ss [BITS_SLICE_THM,SIMP_RULE arith_ss [] (SPECL [`SUC h`,`h`] SLICE_COMP_THM)]
-      ]
-);
-
 val BIT_BITS_LEM = prove(
   `!h l a b. l <= h ==> (BITS h l a = BITS h l b) ==> (BIT h a = BIT h b)`,
-  RW_TAC std_ss [BIT_SLICE,SLICE_THM]
-    THEN PAT_ASSUM `l <= h` (fn th =>
-               ONCE_REWRITE_TAC [GSYM (SIMP_RULE arith_ss [th,SUB_ADD]
-               (SPECL [`h`,`l`,`h-l`,`h-l`] BITS_COMP_THM))])
+  B_RW_TAC [BIT_SLICE,SLICE_THM]
+    THEN PAT_ASSUM `l <= h`
+           (fn th => ONCE_REWRITE_TAC [(GSYM o SIMP_RULE arith_ss [th,SUB_ADD] o
+                                        SPECL [`h`,`l`,`h - l`,`h - l`]) BITS_COMP_THM])
     THEN ASM_REWRITE_TAC []
 );
 
@@ -457,41 +534,29 @@ val BIT_BITS_THM = store_thm("BIT_BITS_THM",
     THEN REPEAT STRIP_TAC
     THENL [
       Cases_on `l = 0`
-        THEN RW_TAC arith_ss [BIT_SLICE,SLICE_THM,EXP,SPEC `0` BITS_ZERO,NOT_ZERO_LT_ZERO],
+        THEN A_RW_TAC [BIT_SLICE,SLICE_THM,EXP,SPEC `0` BITS_ZERO,NOT_ZERO_LT_ZERO],
       EQ_TAC THEN REPEAT STRIP_TAC
         THENL [
-          ONCE_REWRITE_TAC [BITS_SUC]
-            THEN RW_TAC std_ss []
-            THENL [
-               POP_ASSUM (fn th => SIMP_TAC std_ss [SIMP_RULE arith_ss [BIT_SLICE] (SPEC `SUC h` th)]),
-               Cases_on `SUC h < l`
-                 THENL [
-                   RW_TAC std_ss [BITS_ZERO],
-                   RULE_ASSUM_TAC (REWRITE_RULE [NOT_LESS])
-                     THEN PAT_ASSUM `!x. l <= x /\ x <= SUC h ==> (BIT x a = BIT x b)`
-                            (fn th => ASM_SIMP_TAC std_ss [SIMP_RULE arith_ss [BIT_SLICE] (SPEC `SUC h` th)]
-                            THEN ASSUME_TAC th)
-                     THEN POP_ASSUM (fn th => ASSUME_TAC (MATCH_MP
-                           (BETA_RULE (SPECL [`\x. BIT x a = BIT x b`,`l`,`h`] DECEND_LEMMA)) th))
-                     THEN PAT_ASSUM `!l a b.  (!x. l <= x /\ x <= h ==> (BIT x a = BIT x b)) =
-                                              (BITS h l a = BITS h l b)`
-                            (fn th => ASSUME_TAC (SPECL [`l`,`a`,`b`] th))
-                     THEN FULL_SIMP_TAC std_ss []
-                 ]
-            ],
+          B_RW_TAC [BITS_SUC_THM]
+            THEN RULE_ASSUM_TAC (REWRITE_RULE [NOT_LESS])
+            THEN PAT_ASSUM `!x. l <= x /\ x <= SUC h ==> (BIT x a = BIT x b)`
+                   (fn th => ASM_B_SIMP_TAC [SIMP_RULE arith_ss [] (SPEC `SUC h` th)]
+                       THEN ASSUME_TAC (MATCH_MP
+                                 ((BETA_RULE o SPECL [`\x. BIT x a = BIT x b`,`l`,`h`]) DECEND_LEMMA) th))
+            THEN FIRST_ASSUM (fn th => ASSUME_TAC (SPECL [`l`,`a`,`b`] th))
+            THEN B_FULL_SIMP_TAC [],
           IMP_RES_TAC SUB_BITS
-            THEN PAT_ASSUM `!l a b. (!x. l <= x /\ x <= h ==> (BIT x a = BIT x b)) =
-                                    (BITS h l a = BITS h l b)`
-                   (fn th => RULE_ASSUM_TAC (REWRITE_RULE [SYM (SPECL [`l`,`a`,`b`] th)]))
+            THEN FIRST_ASSUM (fn th => RULE_ASSUM_TAC (REWRITE_RULE [SYM (SPECL [`l`,`a`,`b`] th)]))
             THEN Cases_on `x <= h`
-            THEN ASM_SIMP_TAC std_ss []
-            THEN `x = SUC h` by ASM_SIMP_TAC arith_ss []
+            THEN ASM_B_SIMP_TAC []
+            THEN `x = SUC h` by ASM_A_SIMP_TAC []
             THEN Cases_on `l = SUC h`
             THENL [
-              FULL_SIMP_TAC std_ss [BIT_def],
-              `l <= SUC h` by ASM_SIMP_TAC arith_ss []
-                THEN POP_ASSUM (fn th => ASSUME_TAC (SIMP_RULE std_ss [th] (SPECL [`SUC h`,`l`,`a`,`b`] BIT_BITS_LEM)))
-                THEN FULL_SIMP_TAC std_ss []
+              B_FULL_SIMP_TAC [BIT_def],
+              `l <= SUC h` by ASM_A_SIMP_TAC []
+                THEN POP_ASSUM (fn th =>
+                       ASSUME_TAC (SIMP_RULE bool_ss [th] (SPECL [`SUC h`,`l`,`a`,`b`] BIT_BITS_LEM)))
+                THEN B_FULL_SIMP_TAC []
             ]
         ]
     ]
@@ -502,81 +567,135 @@ val BIT_BITS_THM = store_thm("BIT_BITS_THM",
 val BITWISE_LT_2EXP = store_thm("BITWISE_LT_2EXP",
   `!n op a b. BITWISE n op a b < 2 EXP n`,
   Induct_on `n`
-    THEN RW_TAC std_ss [ADD_0,TIMES2,LESS_IMP_LESS_ADD,LESS_MONO_ADD,BITWISE_def,SET_def,EXP]
+    THEN B_RW_TAC [ADD_0,TIMES2,LESS_IMP_LESS_ADD,LESS_MONO_ADD,BITWISE_def,SET_def,EXP]
     THEN REDUCE_TAC
 );
 
 val LESS_EXP_MULT2 = store_thm("LESS_EXP_MULT2",
-  `!a b. a < b ==> ?p. 2 EXP b = 2 EXP (p+1) * 2 EXP a`,
+  `!a b. a < b ==> ?p. 2 EXP b = 2 EXP (p + 1) * 2 EXP a`,
   REPEAT STRIP_TAC
     THEN IMP_RES_TAC LESS_ADD_1
     THEN RULE_ASSUM_TAC (ONCE_REWRITE_RULE [SIMP_RULE arith_ss [] (SPEC `2` (GSYM EXP_INJECTIVE))])
     THEN EXISTS_TAC `p`
     THEN FULL_SIMP_TAC arith_ss [EXP_ADD,MULT_COMM]
 );
-
+ 
 val BITWISE_LEM = store_thm("BITWISE_THM",
   `!n op a b. BIT n (BITWISE (SUC n) op a b) = op (BIT n a) (BIT n b)`,
-  RW_TAC arith_ss [SET_def,BITWISE_def,NOT_BIT]
+  A_RW_TAC [SET_def,BITWISE_def,NOT_BIT]
     THENL [
-       SIMP_TAC arith_ss [BIT_def,BITS_THM,SUC_SUB,SIMP_RULE arith_ss []
-                (SPEC `1` (SIMP_RULE std_ss [BITWISE_LT_2EXP]
-                   (SPECL [`2 EXP n`,`BITWISE n op a b`] DIV_MULT)))],
-       SIMP_TAC arith_ss [BITS_THM,LESS_DIV_EQ_ZERO,BITWISE_LT_2EXP,SUC_SUB]
+       R_SIMP_TAC [BIT_def,BITS_THM,SUC_SUB,
+                  REWRITE_RULE [BITWISE_LT_2EXP] (SPECL [`BITWISE n op a b`,`2 EXP n`] DIV_MULT_1)],
+       R_SIMP_TAC [BITS_THM,LESS_DIV_EQ_ZERO,BITWISE_LT_2EXP,SUC_SUB]
     ]
 );
 
-(* !x. 2 EXP (SUC x - x) = 2 *)
-val TWO_SUC_SUB = GEN_ALL (SIMP_CONV std_ss [SUC_SUB,EXP_1] ``2 EXP (SUC x - x)``);
-
-val LEFT_REWRITE_TAC = GEN_REWRITE_TAC (RATOR_CONV o DEPTH_CONV) empty_rewrites;
+val TWO_SUC_SUB = GEN_ALL (SIMP_CONV bool_ss [SUC_SUB,EXP_1] ``2 EXP (SUC x - x)``);
 
 val BITWISE_THM = store_thm("BITWISE_THM",
   `!x n op a b. x < n ==> (BIT x (BITWISE n op a b) = op (BIT x a) (BIT x b))`,
   Induct_on `n`
     THEN REPEAT STRIP_TAC
     THENL [
-      FULL_SIMP_TAC arith_ss [],
+      A_FULL_SIMP_TAC [],
       Cases_on `x = n`
         THENL [
-           ASM_SIMP_TAC std_ss [BITWISE_LEM],
-           `x < n` by ASM_SIMP_TAC arith_ss []
-              THEN RW_TAC arith_ss [BITWISE_def,SET_def]
+           ASM_REWRITE_TAC [BITWISE_LEM],
+           `x < n` by ASM_A_SIMP_TAC []
+              THEN A_RW_TAC [BITWISE_def,SET_def]
               THEN LEFT_REWRITE_TAC [BIT_def]
-              THEN ASM_SIMP_TAC std_ss [BITS_THM]
+              THEN ASM_REWRITE_TAC [BITS_THM]
               THEN IMP_RES_TAC LESS_EXP_MULT2
               THEN POP_ASSUM (K ALL_TAC)
-              THEN ASM_SIMP_TAC std_ss [ZERO_LT_TWOEXP,ADD_DIV_ADD_DIV,TWO_SUC_SUB,GSYM ADD1,EXP,
-                      ONCE_REWRITE_RULE [MULT_COMM] (REWRITE_RULE [DECIDE(Term`0 < 2`)] (SPEC `2` MOD_TIMES))]
+              THEN ASM_B_SIMP_TAC [ZERO_LT_TWOEXP,ADD_DIV_ADD_DIV,TWO_SUC_SUB,GSYM ADD1,EXP,
+                      ONCE_REWRITE_RULE [MULT_COMM] (REWRITE_RULE [DECIDE (Term `0 < 2`)] (SPEC `2` MOD_TIMES))]
               THEN SUBST_OCCS_TAC [([2],SYM (SPEC `x` TWO_SUC_SUB))]
-              THEN ASM_SIMP_TAC std_ss [GSYM BITS_THM,GSYM BIT_def]
+              THEN ASM_B_SIMP_TAC [GSYM BITS_THM,GSYM BIT_def]
         ]
     ]
 );
 
 val BITWISE_COR = store_thm("BITWISE_COR",
-  `!x n op a b. 
-      x < n ==> 
-      op (BIT x a) (BIT x b) ==> 
-     ((BITWISE n op a b DIV 2 EXP x) MOD 2 = 1)`,
+  `!x n op a b. x < n ==> op (BIT x a) (BIT x b) ==> ((BITWISE n op a b DIV 2 EXP x) MOD 2 = 1)`,
   NTAC 6 STRIP_TAC
     THEN IMP_RES_TAC BITWISE_THM
     THEN NTAC 2 (WEAKEN_TAC (K true))
     THEN POP_ASSUM (fn th => REWRITE_TAC [GSYM th])
-    THEN ASM_SIMP_TAC std_ss 
-    [BITS_THM,BIT_def,DIV1,EXP_1,SUC_SUB]
+    THEN ASM_REWRITE_TAC [BITS_THM,BIT_def,DIV1,EXP_1,SUC_SUB]
 );
  
 val BITWISE_NOT_COR = store_thm("BITWISE_NOT_COR",
-  `!x n op a b. 
-     x < n ==> 
-     ~op (BIT x a) (BIT x b) ==> 
-    ((BITWISE n op a b DIV 2 EXP x) MOD 2 = 0)`,
+  `!x n op a b. x < n ==> ~op (BIT x a) (BIT x b) ==> ((BITWISE n op a b DIV 2 EXP x) MOD 2 = 0)`,
   NTAC 6 STRIP_TAC
     THEN IMP_RES_TAC BITWISE_THM
     THEN NTAC 2 (WEAKEN_TAC (K true))
     THEN POP_ASSUM (fn th => REWRITE_TAC [GSYM th])
-    THEN ASM_SIMP_TAC std_ss [BITS_THM,BIT_def,GSYM NOT_MOD2_LEM,DIV1,EXP_1,SUC_SUB]
+    THEN ASM_REWRITE_TAC [BITS_THM,BIT_def,GSYM NOT_MOD2_LEM,DIV1,EXP_1,SUC_SUB]
+);
+
+(* -------------------------------------------------------- *)
+
+val MOD_PLUS_RIGHT = store_thm("MOD_PLUS_RIGHT",
+ `!n. 0<n ==> !j k. ((j + (k MOD n)) MOD n) = ((j+k) MOD n)`,
+   let fun SUBS th = SUBST_OCCS_TAC [([2],th)]
+   in
+   REPEAT STRIP_TAC THEN
+   IMP_RES_TAC MOD_TIMES THEN
+   PURE_ONCE_REWRITE_TAC [ADD_SYM] THEN
+   IMP_RES_THEN (TRY o SUBS o SPEC (`k:num`)) DIVISION THEN
+   ASM_REWRITE_TAC [SYM(SPEC_ALL ADD_ASSOC)]
+   end);
+
+val MOD_LESS = prove(
+  `!n a. 0 < n ==> a MOD n < n`,
+  PROVE_TAC [DIVISION]
+);
+ 
+val MOD_LESS1 = prove(
+  `!n. 0 < n ==> a MOD n + 1 <= n`,
+  REPEAT STRIP_TAC THEN IMP_RES_TAC MOD_LESS
+    THEN POP_ASSUM (fn th => ASSUME_TAC (SPEC `a` th))
+    THEN A_RW_TAC []
+);
+ 
+val MOD_ZERO = prove(
+  `!n. 0 < n /\ 0 < a /\ a <= n /\ (a MOD n = 0) ==> (a = n)`,
+  REPEAT STRIP_TAC
+    THEN Cases_on `a < n`
+    THEN A_FULL_SIMP_TAC [LESS_MOD,GSYM NOT_ZERO_LT_ZERO]
+);
+ 
+val MOD_PLUS_1 = store_thm("MOD_PLUS_1",
+  `!n. 0 < n ==> !x. ((x + 1) MOD n = 0) = (x MOD n + 1 = n)`,
+  REPEAT STRIP_TAC
+    THEN Cases_on `n = 1`
+    THENL [
+      ASM_A_SIMP_TAC [MOD1],
+      IMP_RES_TAC MOD_PLUS
+        THEN POP_ASSUM (fn th => ONCE_REWRITE_TAC [GSYM th])
+        THEN `1 < n` by ASM_A_SIMP_TAC []
+        THEN ASM_B_SIMP_TAC [LESS_MOD]
+        THEN EQ_TAC THEN STRIP_TAC
+        THENL [
+           `0 < x MOD n + 1` by A_SIMP_TAC []
+             THEN IMP_RES_TAC MOD_LESS1
+             THEN POP_ASSUM (fn th => ASSUME_TAC (SPEC `x` th))
+             THEN IMP_RES_TAC MOD_ZERO,
+           ASM_B_SIMP_TAC [ADD_EQ_SUB,SUB_ADD,DIVMOD_ID]
+        ]
+    ]
+);
+ 
+val MOD_ADD_1 = store_thm("MOD_ADD_1",
+  `!n. 0 < n ==> !x. ~((x + 1) MOD n = 0) ==> ((x + 1) MOD n = x MOD n + 1)`,
+  B_RW_TAC [MOD_PLUS_1]
+    THEN IMP_RES_TAC (SPEC `n` DIVISION)
+    THEN PAT_ASSUM `!k. k = k DIV n * n + k MOD n` (fn th => SUBST_OCCS_TAC [([1],SPEC `x` th)])
+    THEN ONCE_REWRITE_TAC [GSYM ADD_ASSOC]
+    THEN POP_ASSUM (fn th => ASSUME_TAC (SPEC `x` th))
+    THEN `x MOD n + 1 < n` by ASM_A_SIMP_TAC []
+    THEN ASM_B_SIMP_TAC [MOD_TIMES,LESS_MOD]
+ 
 );
 
 (* -------------------------------------------------------- *)
