src/word32/word32Script.sml
@@ -1,20 +1,15 @@
 (* app load ["bossLib","EquivType","pairTheory",
-             "numeralTheory","selectUtil","bitsTheory"]; *)
-
-infix 8 by;
-infix THEN THENC THENL ++;
-
-open HolKernel boolLib selectUtil Q Parse EquivType
-     computeLib bossLib simpLib numLib pairTheory numeralTheory 
-     arithmeticTheory prim_recTheory bitsTheory;
-
+             "numeralTheory","selectUtil","abbrevUtil","bitsTheory"]; *)
  
-(* val arithr_ss = arith_ss++arithSimps.REDUCE_ss; *)
-val arithr_ss = arith_ss;
-val definition = fetch "-";
-
+infix 8 by;
+infix THEN THENC THENL ++ |->;
+ 
+open HolKernel boolLib selectUtil abbrevUtil Q Parse EquivType
+     computeLib bossLib simpLib numLib pairTheory numeralTheory
+     arithmeticTheory prim_recTheory bitsTheory;
+ 
 val PROVE = fn thl => fn q => PROVE thl (Term q);
-  
+ 
 val _ = set_fixity "EQUIVw" (Infixr 450);
 val _ = set_fixity "ADDw" (Infixl 500);
 val _ = set_fixity "SUBw" (Infixl 500);
@@ -23,20 +18,18 @@ val _ = set_fixity "ORw" (Infixl 600);
 val _ = set_fixity "EORw" (Infixl 600);
 val _ = set_fixity "ANDw" (Infixl 650);
 
+val RIGHT_REWRITE_RULE = GEN_REWRITE_RULE (RAND_CONV o DEPTH_CONV) empty_rewrites;
+
 (* -------------------------------------------------------- *)
  
 val _ = new_theory "word32";
 
 (* -------------------------------------------------------- *)
 
-val HB_def = Define`HB = 31`;
-
-val WL_def = Define`WL = SUC HB`;
-
-val WL_POS = REWRITE_RULE [SYM WL_def] (SPEC `HB` LESS_0);
+val HB_def   = Define`HB = 31`;
+val WL_def   = Define`WL = SUC HB`;
 
 val MODw_def = Define`MODw n = n MOD 2 EXP WL`;
-
 val INw_def  = Define`INw n = n < 2 EXP WL`;
 
 val EQUIVw_def = Define`x EQUIVw y = (MODw x = MODw y)`;
@@ -44,11 +37,23 @@ val EQUIVw_def = Define`x EQUIVw y = (MODw x = MODw y)`;
 val EQUIVw_QT = store_thm("EQUIVw_QT",
   `!x y. x EQUIVw y = ($EQUIVw x = $EQUIVw y)`,
   REPEAT STRIP_TAC THEN EQ_TAC
-    THEN RW_TAC std_ss [FUN_EQ_THM,EQUIVw_def,MODw_def]
+    THEN B_RW_TAC [FUN_EQ_THM,EQUIVw_def,MODw_def]
 );
 
 val EQUIVw_RFL = PROVE [EQUIVw_QT] `!x. x EQUIVw x`;
 val EQUIVw_SYM = PROVE [EQUIVw_QT] `!x y. x EQUIVw y = y EQUIVw x`;
+
+(* -------------------------------------------------------- *)
+
+val WL_POS       = REWRITE_RULE [SYM WL_def] (SPEC `HB` LESS_0);
+
+val WL_GEQ_ONE   = prove(`1 <= WL`,A_SIMP_TAC [WL_def,ADD1]);
+
+val WL_SUB_ONE   = SIMP_CONV arith_ss [WL_def] ``WL - 1``;
+
+val WL_SUB_HB    = SIMP_CONV bool_ss [SUC_SUB,WL_def] ``WL - HB``;
+
+val WL_SUB_SUC_X = SIMP_CONV arith_ss [WL_def] ``WL - SUC x``;
 
 (* -------------------------------------------------------- *)
 
@@ -59,140 +64,141 @@ val FUNPOW_THM = store_thm("FUNPOW_THM",
  
 val FUNPOW_THM2 = store_thm("FUNPOW_THM2",
   `!f n x. FUNPOW f (SUC n) x = f (FUNPOW f n x)`,
-  Induct_on `n` THEN RW_TAC std_ss [FUNPOW,FUNPOW_THM]
+  Induct_on `n` THEN B_RW_TAC [FUNPOW,FUNPOW_THM]
 );
 
 val FUNPOW_EVAL = store_thm("FUNPOW_EVAL",
   `!f n x. FUNPOW f n x = if n = 0 then x else FUNPOW f (n-1) (f x)`,
-  Induct_on `n` THEN RW_TAC arith_ss [FUNPOW]
+  Induct_on `n` THEN A_RW_TAC [FUNPOW]
 );
  
 (* -------------------------------------------------------- *)
  
 val INw_MODw = store_thm("INw_MODw",
   `!n. INw (MODw n)`,
-  RW_TAC arith_ss [ZERO_LT_TWOEXP,DIVISION,INw_def,MODw_def]
+  A_RW_TAC [ZERO_LT_TWOEXP,DIVISION,INw_def,MODw_def]
 );
 
 val TOw_IDEM = store_thm("TOw_IDEM",
   `!a. INw a ==> (MODw a = a)`,
-  RW_TAC arith_ss [INw_def,MODw_def,LESS_MOD]
+  A_RW_TAC [INw_def,MODw_def,LESS_MOD]
 );
 
 val MODw_IDEM2 = store_thm("MODw_IDEM2",
   `!a. MODw (MODw a) = MODw a`,
-  RW_TAC std_ss [INw_MODw,TOw_IDEM]
+  B_RW_TAC [INw_MODw,TOw_IDEM]
 );
 
 val TOw_QT = store_thm("TOw_QT",
   `!a. MODw a EQUIVw a`,
-  RW_TAC std_ss [EQUIVw_def,MODw_IDEM2]
+  B_RW_TAC [EQUIVw_def,MODw_IDEM2]
 );
 
 val MODw_THM = store_thm("MODw_THM",
   `MODw = BITS HB 0`,
   ONCE_REWRITE_TAC [FUN_EQ_THM]
-    THEN STRIP_TAC
-    THEN REWRITE_TAC [MODw_def,WL_def,
-       SIMP_CONV arith_ss [WL_def,BITS2_THM,CONJUNCT1 EXP,DIV1] 
-                        ``BITS HB 0 n``]
+    THEN REWRITE_TAC [MODw_def,WL_def,SPEC `HB` BITS_ZERO3]
 );
 
 (* -------------------------------------------------------- *)
  
 val MOD_ADD = store_thm("MOD_ADD",
   `!a b. MODw (a + b) = MODw (MODw a + MODw b)`,
-  RW_TAC std_ss [MODw_def,MOD_PLUS,ZERO_LT_TWOEXP]
+  B_RW_TAC [MODw_def,MOD_PLUS,ZERO_LT_TWOEXP]
 );
 
-val AONE_def = Define`AONE = 1`;
+val MODw_MULT = store_thm("MODw_MULT",
+ `!a b. MODw (a * b) = MODw (MODw a * MODw b)`,
+  B_RW_TAC [MODw_def,MOD_TIMES2,ZERO_LT_TWOEXP]
+);
+
+val AONE_def = Define `AONE = 1`;
 
 val ADD_QT = store_thm("ADD_QT",
   `(!n. 0 + n EQUIVw n) /\ !m n. SUC m + n EQUIVw SUC (m + n)`,
-  RW_TAC arith_ss [EQUIVw_def,ADD]
+  A_RW_TAC [EQUIVw_def,ADD]
 );
 
 val ADD_0_QT = store_thm("ADD_0_QT",
   `!a. a + 0 EQUIVw a`,
-  RW_TAC arith_ss [EQUIVw_def]
+  A_RW_TAC [EQUIVw_def]
 );
 
 val ADD_COMM_QT = store_thm("ADD_COMM_QT",
   `!a b. a + b EQUIVw b + a`,
-  RW_TAC arith_ss [EQUIVw_def]
+  A_RW_TAC [EQUIVw_def]
 );
 
 val ADD_ASSOC_QT = store_thm("ADD_ASSOC_QT",
   `!a b c. a + (b + c) EQUIVw a + b + c`,
-  RW_TAC arith_ss [EQUIVw_def]
+  A_RW_TAC [EQUIVw_def]
 );
 
 val MULT_QT = store_thm("MULT_QT",
   `(!n. 0 * n EQUIVw 0) /\ !m n. SUC m * n EQUIVw m * n + n`,
-  RW_TAC arith_ss [EQUIVw_def,MULT]
+  A_RW_TAC [EQUIVw_def,MULT]
 );
 
 val ADD1_QT = store_thm("ADD1_QT",
   `!m. SUC m EQUIVw m + AONE`,
-  RW_TAC arith_ss [EQUIVw_def,ADD1,AONE_def]
+  A_RW_TAC [EQUIVw_def,ADD1,AONE_def]
 );
 
 val ADD_CLAUSES_QT = store_thm("ADD_CLAUSES_QT",
   `(!m. 0 + m EQUIVw m) /\ (!m. m + 0 EQUIVw m) /\ (!m n. SUC m + n EQUIVw SUC (m + n)) /\
       (!m n. m + SUC n EQUIVw SUC (m + n))`,
-  RW_TAC arith_ss [EQUIVw_def,ADD_CLAUSES]
+  A_RW_TAC [EQUIVw_def,ADD_CLAUSES]
 );
 
-val MODw_0 = SIMP_CONV std_ss [ZERO_LT_TWOEXP,ZERO_MOD,MODw_def] ``MODw 0``;
-val SPEC_MOD_TIMES = REWRITE_RULE [MULT_LEFT_1] (SPEC `1` (SIMP_RULE std_ss [ZERO_LT_TWOEXP]
-                                                (SPEC `2 EXP WL` MOD_TIMES)));
+val MODw_0 = (REWRITE_RULE [GSYM MODw_THM] o SPECL [`HB`,`0`]) BITS_ZERO2;
+val SPEC_MOD_TIMES = (REWRITE_RULE [MULT_LEFT_1] o SPEC `1`
+                        o REWRITE_RULE [ZERO_LT_TWOEXP] o SPEC `2 EXP WL`) MOD_TIMES;
 val exp_gteq = REDUCE_RULE (MATCH_MP TWOEXP_MONO2 (SPEC `WL` ZERO_LESS_EQ));
 
 
 val SUC_EQUIV_COMP = store_thm("SUC_EQUIV_COMP",
   `!a b. SUC a EQUIVw b ==> a EQUIVw (b + (2 EXP WL - 1))`,
-  RW_TAC std_ss [EQUIVw_def]
+  B_RW_TAC [EQUIVw_def]
     THEN ONCE_REWRITE_TAC [MOD_ADD]
     THEN POP_ASSUM (fn th => REWRITE_TAC [SYM th])
-    THEN SIMP_TAC std_ss [MODw_def,GSYM MOD_ADD,ADD1,GSYM LESS_EQ_ADD_SUB,exp_gteq]
-    THEN SIMP_TAC arith_ss [ONCE_REWRITE_RULE [ADD_COMM] SPEC_MOD_TIMES]
+    THEN B_SIMP_TAC [MODw_def,GSYM MOD_ADD,ADD1,GSYM LESS_EQ_ADD_SUB,exp_gteq]
+    THEN A_SIMP_TAC [ONCE_REWRITE_RULE [ADD_COMM] SPEC_MOD_TIMES]
 );
 
 val INV_SUC_EQ_QT = store_thm("INV_SUC_EQ_QT",
   `!m n. (SUC m EQUIVw SUC n) = (m EQUIVw n)`,
-  RW_TAC arith_ss [EQUIVw_def]
+  A_RW_TAC [EQUIVw_def]
     THEN EQ_TAC
     THENL [
-      RW_TAC std_ss []
+      B_RW_TAC []
         THEN IMP_RES_TAC (REWRITE_RULE [EQUIVw_def] SUC_EQUIV_COMP)
-        THEN FULL_SIMP_TAC arithr_ss [GSYM LESS_EQ_ADD_SUB,ADD1,MODw_def,exp_gteq]
+        THEN R_FULL_SIMP_TAC [GSYM LESS_EQ_ADD_SUB,ADD1,MODw_def,exp_gteq]
         THEN REWRITE_TAC [ONCE_REWRITE_RULE [ADD_COMM] SPEC_MOD_TIMES],
       REWRITE_TAC [ADD1]
         THEN ONCE_REWRITE_TAC [MOD_ADD]
-        THEN RW_TAC std_ss []
+        THEN B_RW_TAC []
     ]
 );
 
 val ADD_INV_0_QT = store_thm("ADD_INV_0_QT",
   `!m n. (m + n EQUIVw m) ==> (n EQUIVw 0)`,
   Induct_on `m`
-    THEN RW_TAC std_ss [ADD_CLAUSES]
-    THEN FULL_SIMP_TAC std_ss [INV_SUC_EQ_QT]
+    THEN B_RW_TAC [ADD_CLAUSES]
+    THEN B_FULL_SIMP_TAC [INV_SUC_EQ_QT]
 );
 
 val ADD_INV_0_EQ_QT = store_thm("ADD_INV_0_EQ_QT",
   `!m n. (m + n EQUIVw m) = (n EQUIVw 0)`,
   REPEAT STRIP_TAC THEN EQ_TAC THEN STRIP_TAC
     THEN IMP_RES_TAC ADD_INV_0_QT
-    THEN FULL_SIMP_TAC std_ss [EQUIVw_def]
+    THEN B_FULL_SIMP_TAC [EQUIVw_def]
     THEN ONCE_REWRITE_TAC [MOD_ADD]
-    THEN ASM_SIMP_TAC arith_ss [MODw_0,MODw_IDEM2]
+    THEN ASM_A_SIMP_TAC [MODw_0,MODw_IDEM2]
 );
 
 val EQ_ADD_LCANCEL_QT = store_thm("EQ_ADD_LCANCEL_QT",
   `!m n p. (m + n EQUIVw m + p) = (n EQUIVw p)`,
-  Induct_on `m`
-    THEN ASM_REWRITE_TAC [ADD_CLAUSES,INV_SUC_EQ_QT]
+  Induct_on `m` THEN ASM_REWRITE_TAC [ADD_CLAUSES,INV_SUC_EQ_QT]
 );
 
 val EQ_ADD_RCANCEL_QT = store_thm("EQ_ADD_RCANCEL_QT",
@@ -202,23 +208,23 @@ val EQ_ADD_RCANCEL_QT = store_thm("EQ_ADD_RCANCEL_QT",
 
 val LEFT_ADD_DISTRIB_QT = store_thm("LEFT_ADD_DISTRIB_QT",
   `!m n p. p * (m + n) EQUIVw p * m + p * n`,
-  RW_TAC arith_ss [EQUIVw_def,LEFT_ADD_DISTRIB]
+  A_RW_TAC [EQUIVw_def,LEFT_ADD_DISTRIB]
 );
 
 val MULT_ASSOC_QT = store_thm("MULT_ASSOC_QT",
   `!m n p. m * (n * p) EQUIVw m * n * p`,
-  RW_TAC arith_ss [EQUIVw_def,MULT_ASSOC]
+  A_RW_TAC [EQUIVw_def,MULT_ASSOC]
 );
 
 val MULT_COMM_QT = store_thm("MULT_COMM_QT",
   `!m n. m * n EQUIVw n * m`,
-  RW_TAC arith_ss [EQUIVw_def,MULT_COMM]
+  A_RW_TAC [EQUIVw_def,MULT_COMM]
 );
 
 val MULT_CLAUSES_QT = store_thm("MULT_CLAUSES_QT",
   `!m n. (0 * m EQUIVw 0) /\ (m * 0 EQUIVw 0) /\ (AONE * m EQUIVw m) /\ (m * AONE EQUIVw m) /\
          (SUC m * n EQUIVw m * n + n) /\ (m * SUC n EQUIVw m + m * n)`,
-  RW_TAC arith_ss [EQUIVw_def,MULT_CLAUSES,AONE_def]
+  A_RW_TAC [EQUIVw_def,MULT_CLAUSES,AONE_def]
 );
 
 (* -------------------------------------------------------- *)
@@ -231,12 +237,10 @@ val MODw_LESS = REWRITE_RULE [MODw_def,INw_def] INw_MODw;
 
 val ADD_TWO_COMP_QT = store_thm("ADD_TWO_COMP_QT",
   `!a. MODw a + TWO_COMP a EQUIVw 0`,
-  RW_TAC arith_ss [TWO_COMP_def,EQUIVw_def,MODw_def]
+  A_RW_TAC [TWO_COMP_def,EQUIVw_def,MODw_def]
    THEN ASSUME_TAC (SPEC `a` MODw_LESS)
    THEN IMP_RES_TAC LESS_IMP_LESS_OR_EQ
-   THEN ASM_SIMP_TAC std_ss [GSYM LESS_EQ_ADD_SUB]
-   THEN ONCE_REWRITE_TAC [ADD_COMM]
-   THEN SIMP_TAC std_ss [ADD_SUB,ZERO_MOD,DIVMOD_ID,ZERO_LT_TWOEXP]
+   THEN ASM_A_SIMP_TAC [GSYM LESS_EQ_ADD_SUB,ADD_SUB,ZERO_MOD,DIVMOD_ID,ZERO_LT_TWOEXP]
 );
  
 val TWO_COMP_ONE_COMP_QT = store_thm("TWO_COMP_ONE_COMP_QT",
@@ -244,63 +248,62 @@ val TWO_COMP_ONE_COMP_QT = store_thm("TWO_COMP_ONE_COMP_QT",
   STRIP_TAC THEN REWRITE_TAC [AONE_def]
     THEN ASSUME_TAC (SPEC `a` (REWRITE_RULE [INw_def] INw_MODw))
     THEN `1 + MODw a <= 2 EXP WL` by DECIDE_TAC
-    THEN RW_TAC arith_ss [EQUIVw_def,ONE_COMP_def,TWO_COMP_def,SUB_RIGHT_SUB,SUB_RIGHT_ADD]
+    THEN A_RW_TAC [EQUIVw_def,ONE_COMP_def,TWO_COMP_def,SUB_RIGHT_SUB,SUB_RIGHT_ADD]
     THEN Cases_on `1 + MODw a = 2 EXP WL`
     THENL [
-      RULE_ASSUM_TAC (SIMP_RULE std_ss [GSYM SUC_ONE_ADD,GSYM PRE_SUC_EQ,ZERO_LT_TWOEXP])
-        THEN ASM_SIMP_TAC arithr_ss [MODw_def,PRE_SUB1],
-      FULL_SIMP_TAC arithr_ss []
+      RULE_ASSUM_TAC (SIMP_RULE bool_ss [GSYM SUC_ONE_ADD,GSYM PRE_SUC_EQ,ZERO_LT_TWOEXP])
+        THEN ASM_R_SIMP_TAC [MODw_def,PRE_SUB1],
+      R_FULL_SIMP_TAC []
     ]
 );
 
 (* -------------------------------------------------------- *)
 
-(* !h n. BITS h 0 n = n MOD 2 EXP SUC h *)
-val BITS_COR = GEN_ALL (SIMP_RULE arithr_ss [DIV1] (SPECL [`h`,`0`] BITS2_THM));
- 
-(* !n a b. (!x. x <= n ==> (BIT x a = BIT x b)) = (BITS n 0 a = BITS n 0 b) *)
-val BIT_BITS_THM_0 = GEN `n` (SIMP_RULE arith_ss [] (SPECL [`n`,`0`] BIT_BITS_THM));
- 
-(* BIT_EQUIV_THM: |- !a b. (!x. x < WL ==> (BIT x a = BIT x b)) = a EQUIVw b *)
+(* |- !n a b. (!x. x <= n ==> (BIT x a = BIT x b)) = (BITS n 0 a = BITS n 0 b) *)
+val BIT_BITS_THM_0 = (GEN `n` o SIMP_RULE arith_ss [] o SPECL [`n`,`0`]) BIT_BITS_THM;
+
+(* |- !a b. (!x. x < WL ==> (BIT x a = BIT x b)) = a EQUIVw b *)
 val BIT_EQUIV_THM = save_thm("BIT_EQUIV_THM",
-   SIMP_RULE std_ss [BITS_COR,GSYM MODw_def,GSYM WL_def,GSYM EQUIVw_def,LESS_EQ_IMP_LESS_SUC,
-            REWRITE_RULE [GSYM LESS_EQ,GSYM WL_def] (ONCE_REWRITE_CONV [GSYM LESS_EQ_MONO] ``x <= HB``)]
-                (SPEC `HB` BIT_BITS_THM_0)
+   SIMP_RULE bool_ss [BITS_ZERO3,GSYM MODw_def,GSYM WL_def,GSYM EQUIVw_def,LESS_EQ_IMP_LESS_SUC,
+                REWRITE_RULE [GSYM LESS_EQ,GSYM WL_def] (ONCE_REWRITE_CONV [GSYM LESS_EQ_MONO] ``x <= HB``)]
+                    (SPEC `HB` BIT_BITS_THM_0)
 );
 
 (* -------------------------------------------------------- *)
 
-val SLICE_COR = GEN_ALL (SIMP_RULE arithr_ss [] (SPECL [`n`,`h`,`0`] SLICE_THM));
+(* |- !n h. SLICE h 0 n = BITS h 0 n *)
+val SLICE_COR = (GEN_ALL o SIMP_RULE arithr_ss [] o SPECL [`n`,`h`,`0`]) SLICE_THM;
  
 val BITS_SUC2 = store_thm("BITS_SUC2",
   `!n a. BITS (SUC n) 0 a = SLICE (SUC n) (SUC n) a + BITS n 0 a`,
-  RW_TAC arith_ss [GSYM SLICE_COR,SLICE_COMP_THM]
+  A_RW_TAC [GSYM SLICE_COR,SLICE_COMP_THM]
 );
- 
-val lemma1 = prove(
+
+val lem = prove(
   `!n a. a < 2 EXP SUC n ==> ~(2 EXP SUC n < a + 1)`,
-  RW_TAC arith_ss [NOT_LESS,EXP]
+  A_RW_TAC [NOT_LESS,EXP]
 );
+
+val lem2 = MATCH_MP lem (REWRITE_RULE [SUB_0] (SPECL [`n`,`0`,`a`] BITSLT_THM));
 
 val BITWISE_ONE_COMP_LEM = prove(
   `!n a b. BITWISE (SUC n) (\x y. ~x) a b = 2 EXP (SUC n) - 1 - BITS n 0 a`,
   Induct_on `n`
     THEN REPEAT STRIP_TAC
     THENL [
-      RW_TAC arithr_ss [SET_def,BIT_def,BITWISE_def,GSYM NOT_BITS],
-      RW_TAC arith_ss [BITWISE_def,SET_def,REWRITE_RULE [SLICE_THM] BITS_SUC2]
-        THEN RULE_ASSUM_TAC (SIMP_RULE std_ss [NOT_BIT,NOT_BITS,BIT_def])
-        THEN ASM_SIMP_TAC arith_ss [MULT_CLAUSES]
+      R_RW_TAC [SET_def,BIT_def,BITWISE_def,NOT_BITS2],
+      A_RW_TAC [BITWISE_def,SET_def,REWRITE_RULE [SLICE_THM] BITS_SUC2]
+        THEN RULE_ASSUM_TAC (SIMP_RULE bool_ss [NOT_BIT,NOT_BITS,BIT_def])
+        THEN ASM_A_SIMP_TAC [MULT_CLAUSES]
         THENL [
            Cases_on `2 EXP SUC n = BITS n 0 a + 1`
              THENL [
-               ASM_SIMP_TAC arith_ss [SUB_RIGHT_ADD,EXP],
-               ASSUME_TAC (SIMP_RULE std_ss [SIMP_RULE arith_ss [] (SPECL [`n`,`0`] BITSLT_THM)]
-                             (SPECL [`n`,`BITS n 0 a`] lemma1))
-                 THEN `~(2 EXP SUC n <= BITS n 0 a + 1)` by ASM_SIMP_TAC arith_ss []
-                 THEN ASM_SIMP_TAC arith_ss [SUB_RIGHT_ADD,EXP]
+               ASM_A_SIMP_TAC [SUB_RIGHT_ADD,EXP],
+               ASSUME_TAC lem2
+                 THEN `~(2 EXP SUC n <= BITS n 0 a + 1)` by ASM_A_SIMP_TAC []
+                 THEN ASM_A_SIMP_TAC [SUB_RIGHT_ADD,EXP]
              ],
-           SIMP_TAC std_ss [REWRITE_CONV [ADD_SUB,TIMES2] ``2 * a - a``,SUB_PLUS,EXP]
+           REWRITE_TAC [REWRITE_CONV [ADD_SUB,TIMES2] ``2 * a - a``,SUB_PLUS,EXP]
         ]
     ]
 );
@@ -309,17 +312,17 @@ val BITWISE_ONE_COMP_LEM = prove(
 
 val BITWISE_ONE_COMP_THM = store_thm("BITWISE_ONE_COMP_THM",
   `!a b. BITWISE WL (\x y. ~x) a b = ONE_COMP a`,
-  RW_TAC std_ss [WL_def,SPEC `HB` BITWISE_ONE_COMP_LEM,ONE_COMP_def,MODw_THM]
+  B_RW_TAC [WL_def,SPEC `HB` BITWISE_ONE_COMP_LEM,ONE_COMP_def,MODw_THM]
 );
 
 val ONE_COMP_THM = store_thm("ONE_COMP_THM",
   `!a x. x < WL ==> (BIT x (ONE_COMP a) = ~BIT x a)`,
-  REWRITE_TAC [GSYM BITWISE_ONE_COMP_THM] THEN RW_TAC std_ss [BITWISE_THM]
+  REWRITE_TAC [GSYM BITWISE_ONE_COMP_THM] THEN B_RW_TAC [BITWISE_THM]
 );
 
 val ZERO_IS_FALSE = prove(
   `!x. ~BIT x 0`,
-  RW_TAC arith_ss [BIT_def,BITS_THM,ZERO_LT_TWOEXP,ZERO_DIV,ZERO_MOD]
+  A_RW_TAC [BIT_def,BITS_THM,ZERO_LT_TWOEXP,ZERO_DIV,ZERO_MOD]
 );
 
 (* ONE_COMP_TRUE: |- !x. x < WL ==> BIT x (ONE_COMP 0) *)
@@ -328,100 +331,97 @@ val ONE_COMP_TRUE = REWRITE_RULE [ZERO_IS_FALSE] (SPEC `0` ONE_COMP_THM);
 (* -------------------------------------------------------- *)
 
 val OR_def    = Define `OR = BITWISE WL $\/`;
-
 val AND_def   = Define `AND = BITWISE WL $/\`;
-
 val EOR_def   = Define `EOR = BITWISE WL (\x y. ~(x = y))`;
-
-val ATRUE_def = Define `ATRUE = ONE_COMP 0`;
+val COMP0_def = Define `COMP0 = ONE_COMP 0`;
 
 (* -------------------------------------------------------- *)
 
 val BITWISE_THM2 = save_thm("BITWISE_THM2",
   (GEN `y` o GEN `op` o GEN `a` o GEN `b`)
-  (SIMP_RULE std_ss [BITWISE_THM] (SPECL [`BITWISE WL op a b`,`y`] BIT_EQUIV_THM))
+  (SIMP_RULE bool_ss [BITWISE_THM] (SPECL [`BITWISE WL op a b`,`y`] BIT_EQUIV_THM))
 );
 
 val OR_ASSOC_QT = save_thm("OR_ASSOC_QT",
   (GEN `a` o GEN `b` o GEN `c`)
-  (SIMP_RULE std_ss [BITWISE_THM,DISJ_ASSOC,GSYM OR_def]
+  (SIMP_RULE bool_ss [BITWISE_THM,DISJ_ASSOC,GSYM OR_def]
   (SPECL [`BITWISE WL $\/ (BITWISE WL $\/ a b) c`,`$\/`,`a`,`BITWISE WL $\/ b c`] BITWISE_THM2))
 );
 
 val OR_COMM_QT = save_thm("OR_COMM_QT",
   (GEN `a` o GEN `b`)
-  (SIMP_RULE std_ss [BITWISE_THM,DISJ_COMM,GSYM OR_def]
+  (SIMP_RULE bool_ss [BITWISE_THM,DISJ_COMM,GSYM OR_def]
   (SPECL [`BITWISE WL ($\/) b a`,`$\/`,`a`,`b`] BITWISE_THM2))
 );
 
 val OR_ABSORB_QT = save_thm("OR_ABSORB_QT",
   (GEN `a` o GEN `b`)
-  (SIMP_RULE std_ss [BITWISE_THM,PROVE [] `!a b. a /\ (a \/ b) = a`,GSYM OR_def,GSYM AND_def]
+  (SIMP_RULE bool_ss [BITWISE_THM,PROVE [] `!a b. a /\ (a \/ b) = a`,GSYM OR_def,GSYM AND_def]
   (SPECL [`a`,`$/\`,`a`,`BITWISE WL $\/ a b`] BITWISE_THM2))
 );
 
 val OR_IDEM_QT = save_thm("OR_IDEM_QT",
-  GEN_ALL (SIMP_RULE std_ss [OR_CLAUSES,GSYM OR_def] (SPECL [`a`,`$\/`,`a`,`a`] BITWISE_THM2))
+  GEN_ALL (SIMP_RULE bool_ss [OR_CLAUSES,GSYM OR_def] (SPECL [`a`,`$\/`,`a`,`a`] BITWISE_THM2))
 );
 
 val AND_ASSOC_QT = save_thm("AND_ASSOC_QT",
   (GEN `a` o GEN `b` o GEN `c`)
-  (SIMP_RULE std_ss [BITWISE_THM,CONJ_ASSOC,GSYM AND_def]
+  (SIMP_RULE bool_ss [BITWISE_THM,CONJ_ASSOC,GSYM AND_def]
   (SPECL [`BITWISE WL $/\ (BITWISE WL $/\ a b) c`,`$/\`,`a`,`BITWISE WL $/\ b c`] BITWISE_THM2))
 );
 
 val AND_COMM_QT = save_thm("AND_COMM_QT",
   (GEN `a` o GEN `b`)
-  (SIMP_RULE std_ss [BITWISE_THM,CONJ_COMM,GSYM AND_def]
+  (SIMP_RULE bool_ss [BITWISE_THM,CONJ_COMM,GSYM AND_def]
   (SPECL [`BITWISE WL $/\ b a`,`$/\`,`a`,`b`] BITWISE_THM2))
 );
 
 val AND_ABSORB_QT = save_thm("AND_ABSORB_QT",
   (GEN `a` o GEN `b`)
-  (SIMP_RULE std_ss [BITWISE_THM,PROVE [] `!a b. a \/ (a /\ b) = a`,GSYM AND_def,GSYM OR_def]
+  (SIMP_RULE bool_ss [BITWISE_THM,PROVE [] `!a b. a \/ (a /\ b) = a`,GSYM AND_def,GSYM OR_def]
   (SPECL [`a`,`$\/`,`a`,`BITWISE WL $/\ a b`] BITWISE_THM2))
 );
 
 val AND_IDEM_QT = save_thm("AND_IDEM_QT",
-  GEN_ALL (SIMP_RULE std_ss [AND_CLAUSES,GSYM AND_def] (SPECL [`a`,`$/\`,`a`,`a`] BITWISE_THM2))
+  GEN_ALL (SIMP_RULE bool_ss [AND_CLAUSES,GSYM AND_def] (SPECL [`a`,`$/\`,`a`,`a`] BITWISE_THM2))
 );
 
 val OR_COMP_QT = save_thm("OR_COMP_QT",
-  GEN_ALL (SIMP_RULE std_ss [EXCLUDED_MIDDLE,ONE_COMP_TRUE,ONE_COMP_THM,GSYM OR_def,GSYM ATRUE_def]
+  GEN_ALL (SIMP_RULE bool_ss [EXCLUDED_MIDDLE,ONE_COMP_TRUE,ONE_COMP_THM,GSYM OR_def,GSYM COMP0_def]
           (SPECL [`ONE_COMP 0`,`$\/`,`a`,`ONE_COMP a`] BITWISE_THM2))
 );
 
 val AND_COMP_QT = save_thm("AND_COMP_QT",
-  GEN_ALL (SIMP_RULE std_ss [ONE_COMP_THM,ZERO_IS_FALSE,GSYM AND_def]
+  GEN_ALL (SIMP_RULE bool_ss [ONE_COMP_THM,ZERO_IS_FALSE,GSYM AND_def]
           (SPECL [`0`,`$/\`,`a`,`ONE_COMP a`] BITWISE_THM2))
 );
 
 val ONE_COMP_QT = save_thm("ONE_COMP_QT",
-  GEN_ALL (SIMP_RULE std_ss [BITWISE_ONE_COMP_THM,ONE_COMP_THM]
+  GEN_ALL (SIMP_RULE bool_ss [BITWISE_ONE_COMP_THM,ONE_COMP_THM]
           (SPECL [`a`,`\x y. ~x`,`ONE_COMP a`,`b`] BITWISE_THM2))
 );
 
 val RIGHT_AND_OVER_OR_QT = save_thm("RIGHT_AND_OVER_OR_QT",
   (GEN `a` o GEN `b` o GEN `c`)
-  (SIMP_RULE std_ss [BITWISE_THM,RIGHT_AND_OVER_OR,GSYM AND_def,GSYM OR_def]
+  (SIMP_RULE bool_ss [BITWISE_THM,RIGHT_AND_OVER_OR,GSYM AND_def,GSYM OR_def]
   (SPECL [`BITWISE WL $\/ (BITWISE WL $/\ a c) (BITWISE WL $/\ b c)`,
           `$/\`,`BITWISE WL $\/ a b`,`c`] BITWISE_THM2))
 );
 
 val RIGHT_OR_OVER_AND_QT = save_thm("RIGHT_OR_OVER_AND_QT",
   (GEN `a` o GEN `b` o GEN `c`)
-  (SIMP_RULE std_ss [BITWISE_THM,RIGHT_OR_OVER_AND,GSYM AND_def,GSYM OR_def]
+  (SIMP_RULE bool_ss [BITWISE_THM,RIGHT_OR_OVER_AND,GSYM AND_def,GSYM OR_def]
   (SPECL [`BITWISE WL $/\ (BITWISE WL $\/ a c) (BITWISE WL $\/ b c)`,
           `$\/`,`BITWISE WL $/\ a b`,`c`] BITWISE_THM2))
 );
 
 val DE_MORGAN_THM_QT1 = 
-  (SIMP_RULE std_ss [BITWISE_THM,BITWISE_ONE_COMP_THM,ONE_COMP_THM,GSYM AND_def,GSYM OR_def]
+  (SIMP_RULE bool_ss [BITWISE_THM,BITWISE_ONE_COMP_THM,ONE_COMP_THM,GSYM AND_def,GSYM OR_def]
   (SPECL [`ONE_COMP (BITWISE WL $/\ a b)`,
           `$\/`,`ONE_COMP a`,`ONE_COMP b`] BITWISE_THM2));
 
 val DE_MORGAN_THM_QT2 = 
-  (SIMP_RULE std_ss [BITWISE_THM,BITWISE_ONE_COMP_THM,ONE_COMP_THM,GSYM AND_def,GSYM OR_def]
+  (SIMP_RULE bool_ss [BITWISE_THM,BITWISE_ONE_COMP_THM,ONE_COMP_THM,GSYM AND_def,GSYM OR_def]
   (SPECL [`ONE_COMP (BITWISE WL $\/ a b)`,
           `$/\`,`ONE_COMP a`,`ONE_COMP b`] BITWISE_THM2));
 
@@ -435,7 +435,7 @@ val DE_MORGAN_THM_QT = save_thm("DE_MORGAN_THM_QT",
 
 val BIT_EQUIV = store_thm("BIT_EQUIV",
   `!n a b. n < WL ==> a EQUIVw b ==> (BIT n a = BIT n b)`,
-  RW_TAC std_ss [GSYM BIT_EQUIV_THM]
+  B_RW_TAC [GSYM BIT_EQUIV_THM]
 );
 
 (* -------------------------------------------------------- *)
@@ -444,12 +444,12 @@ val HB_LESS_WL = REWRITE_RULE [SYM WL_def] (SPEC `HB` LESS_SUC_REFL);
 
 val LSB_WELLDEF = store_thm("LSB_WELLDEF",
   `!a b. a EQUIVw b ==> (LSB a = LSB b)`,
-  RW_TAC std_ss [WL_POS,REDUCE_RULE (SPEC `0` BIT_EQUIV),LSB_def]
+  B_RW_TAC [WL_POS,REDUCE_RULE (SPEC `0` BIT_EQUIV),LSB_def]
 );
 
 val MSB_WELLDEF = store_thm("MSB_WELLDEF",
   `!a b. a EQUIVw b ==> (MSB a = MSB b)`,
-  RW_TAC std_ss [HB_LESS_WL,REDUCE_RULE (SPEC `HB` BIT_EQUIV),MSB_def]
+  B_RW_TAC [HB_LESS_WL,REDUCE_RULE (SPEC `HB` BIT_EQUIV),MSB_def]
 );
 
 (* -------------------------------------------------------- *)
@@ -458,77 +458,76 @@ val BIT_SET_NOT_ZERO = prove(
   `!a. (a MOD 2 = 1) ==> (1 <= a)`,
   SPOSE_NOT_THEN STRIP_ASSUME_TAC
     THEN `a = 0` by DECIDE_TAC
-    THEN FULL_SIMP_TAC arith_ss [ZERO_MOD]
+    THEN A_FULL_SIMP_TAC [ZERO_MOD]
 );
 
 val BIT_SET_NOT_ZERO_COR = prove(
   `!x n op a b. x < n ==> op (BIT x a) (BIT x b) ==> (1 <= (BITWISE n op a b DIV 2 EXP x))`,
-  REPEAT STRIP_TAC THEN ASM_SIMP_TAC std_ss [BITWISE_COR,BIT_SET_NOT_ZERO]
+  REPEAT STRIP_TAC THEN ASM_B_SIMP_TAC [BITWISE_COR,BIT_SET_NOT_ZERO]
 );
 
 val BIT_SET_NOT_ZERO_COR2 = REWRITE_RULE [DIV1,EXP] (SPEC `0` BIT_SET_NOT_ZERO_COR);
 
-val ADD_DIV_ADD_DIV2 = ONCE_REWRITE_RULE [MULT_COMM] (SIMP_RULE arith_ss [] (SPEC `2` ADD_DIV_ADD_DIV))
- 
+val ADD_DIV_ADD_DIV2 = ONCE_REWRITE_RULE [MULT_COMM] (SIMP_RULE arith_ss [] (SPEC `2` ADD_DIV_ADD_DIV));
+
 val BIT_DIV2 = prove(
   `!i. BIT n (i DIV 2) = BIT (SUC n) i`,
-  RW_TAC arithr_ss [BIT_def,BITS_THM,EXP,ZERO_LT_TWOEXP,DIV_DIV_DIV_MULT]
+  R_RW_TAC [BIT_def,BITS_THM,EXP,ZERO_LT_TWOEXP,DIV_DIV_DIV_MULT]
 );
- 
+
 val lemma1 = prove(
   `!a b n. 0 < n ==> ((a + SET b n) DIV 2 = a DIV 2 + SET b (n - 1))`,
-  RW_TAC arith_ss [SET_def]
+  A_RW_TAC [SET_def]
     THEN IMP_RES_TAC LESS_ADD_1
-    THEN FULL_SIMP_TAC arith_ss [GSYM ADD1,ADD_DIV_ADD_DIV2,EXP]
+    THEN A_FULL_SIMP_TAC [GSYM ADD1,ADD_DIV_ADD_DIV2,EXP]
 );
- 
+
 val lemma2 = prove(
   `!b n. 2 * (SET b n) = SET b (n + 1)`,
-  RW_TAC std_ss [MULT_CLAUSES,SET_def,GSYM ADD1,EXP]
+  B_RW_TAC [MULT_CLAUSES,SET_def,GSYM ADD1,EXP]
 );
- 
+
 val lemma3 = prove(
   `!n op a b. 0 < n ==> (BITWISE n op a b MOD 2 = SET (op (LSB a) (LSB b)) 0)`,
-  RW_TAC std_ss [LSB_def]
-    THEN POP_ASSUM (fn th => ONCE_REWRITE_TAC [SIMP_RULE std_ss [th]
-                               ((GSYM o SPECL [`0`,`n`,`op`,`a`,`b`]) BITWISE_THM)])
-    THEN RW_TAC std_ss [GSYM LSB_def,LSB_ODD,ODD_MOD2_LEM,SET_def,EXP]
-    THEN FULL_SIMP_TAC std_ss [GSYM NOT_MOD2_LEM]
+  B_RW_TAC [LSB_def]
+    THEN POP_ASSUM (fn th => ONCE_REWRITE_TAC [MATCH_MP ((GSYM o SPEC `0`) BITWISE_THM) th])
+    THEN B_RW_TAC [GSYM LSB_def,LSB_ODD,ODD_MOD2_LEM,SET_def,EXP]
+    THEN B_FULL_SIMP_TAC [GSYM NOT_MOD2_LEM]
 );
 
 val lemma4 = prove(
   `!n op a b. 0 < n /\ BITWISE n op a b <= SET (op (LSB a) (LSB b)) 0 ==>
               (BITWISE n op a b = SET (op (LSB a) (LSB b)) 0)`,
-  RW_TAC arith_ss [LSB_def,SET_def,EXP]
+  A_RW_TAC [LSB_def,SET_def,EXP]
     THEN IMP_RES_TAC BIT_SET_NOT_ZERO_COR2
-    THEN ASM_SIMP_TAC arith_ss []
+    THEN ASM_A_SIMP_TAC []
 );
- 
+
 val BITWISE_ISTEP = store_thm("BITWISE_ISTEP",
   `!n op a b. 0 < n ==> (BITWISE n op (a DIV 2) (b DIV 2) =
                         (BITWISE n op a b) DIV 2 + SET (op (BIT n a) (BIT n b)) (n - 1))`,
   Induct_on `n`
     THEN REPEAT STRIP_TAC
     THENL [
-       FULL_SIMP_TAC arith_ss [],
+       A_FULL_SIMP_TAC [],
        Cases_on `n = 0`
          THENL [
-            RW_TAC arithr_ss [BITWISE_def,SET_def,BIT_DIV2],
-            FULL_SIMP_TAC std_ss [NOT_ZERO_LT_ZERO,BITWISE_def,SUC_SUB1,BIT_DIV2,lemma1]
+            R_RW_TAC [BITWISE_def,SET_def,BIT_DIV2],
+            B_FULL_SIMP_TAC [NOT_ZERO_LT_ZERO,BITWISE_def,SUC_SUB1,BIT_DIV2,lemma1]
          ]
     ]
 );
 
-val BITWISE_EVAL = store_thm("BITWISE_def2",
+val BITWISE_EVAL = store_thm("BITWISE_EVAL",
   `!n op a b. BITWISE (SUC n) op a b =
          2 * (BITWISE n op (a DIV 2) (b DIV 2)) + SET (op (LSB a) (LSB b)) 0`,
   REPEAT STRIP_TAC
     THEN Cases_on `n = 0`
     THENL [
-       RW_TAC arith_ss [BITWISE_def,MULT_CLAUSES,LSB_def],
-       FULL_SIMP_TAC arith_ss [BITWISE_def,NOT_ZERO_LT_ZERO,BITWISE_ISTEP,
-                               DIV_MULT_THM2,LEFT_ADD_DISTRIB,SUB_ADD,lemma2,lemma3]
-         THEN RW_TAC arith_ss [SUB_RIGHT_ADD,lemma4]
+       A_RW_TAC [BITWISE_def,MULT_CLAUSES,LSB_def],
+       A_FULL_SIMP_TAC [BITWISE_def,NOT_ZERO_LT_ZERO,BITWISE_ISTEP,
+                        DIV_MULT_THM2,LEFT_ADD_DISTRIB,SUB_ADD,lemma2,lemma3]
+         THEN A_RW_TAC [SUB_RIGHT_ADD,lemma4]
     ]
 );
 
@@ -536,41 +535,39 @@ val BITWISE_EVAL = store_thm("BITWISE_def2",
 
 val MODw_2EXP_GT_WL = prove(
   `!n. WL <= n ==> (MODw (2 EXP n) = 0)`,
-  RW_TAC std_ss [MODw_def]
+  B_RW_TAC [MODw_def]
     THEN IMP_RES_TAC LESS_EQ_EXP_MULT
-    THEN ASM_SIMP_TAC std_ss [ZERO_LT_TWOEXP,MOD_EQ_0]
+    THEN ASM_B_SIMP_TAC [ZERO_LT_TWOEXP,MOD_EQ_0]
 );
- 
+
 val BITWISE_WELLDEF = store_thm("BITWISE_WELLDEF",
   `!n op a b c d. a EQUIVw b /\ c EQUIVw d ==> (BITWISE n op) a c EQUIVw (BITWISE n op) b d`,
   Induct_on `n`
     THEN REPEAT STRIP_TAC
     THENL [
-       SIMP_TAC arith_ss [BITWISE_def,EQUIVw_def],
-       PAT_ASSUM `!op a b c d.  a EQUIVw b /\ c EQUIVw d ==>
-                                BITWISE n op a c EQUIVw BITWISE n op b d`
-            (fn th => `!op. BITWISE n op a c EQUIVw BITWISE n op b d` by
+       A_SIMP_TAC [BITWISE_def,EQUIVw_def],
+       FIRST_ASSUM (fn th => `!op. BITWISE n op a c EQUIVw BITWISE n op b d` by
                         IMP_RES_TAC (SPECL [`op`,`a`,`b`,`c`,`d`] th))
-         THEN ASM_SIMP_TAC std_ss [BITWISE_def]
+         THEN ASM_B_SIMP_TAC [BITWISE_def]
          THEN Cases_on `n < WL`
          THENL [
             IMP_RES_TAC BIT_EQUIV THEN NTAC 4 (POP_ASSUM (K ALL_TAC))
-              THEN RW_TAC arith_ss [SET_def]
-              THEN FULL_SIMP_TAC std_ss [EQUIVw_def]
+              THEN A_RW_TAC [SET_def]
+              THEN B_FULL_SIMP_TAC [EQUIVw_def]
               THEN ONCE_REWRITE_TAC [MOD_ADD]
-              THEN ASM_SIMP_TAC std_ss [],
+              THEN ASM_B_SIMP_TAC [],
             RULE_ASSUM_TAC (REWRITE_RULE [NOT_LESS])
-              THEN RW_TAC arith_ss [SET_def]
-              THEN FULL_SIMP_TAC std_ss [EQUIVw_def]
+              THEN A_RW_TAC [SET_def]
+              THEN B_FULL_SIMP_TAC [EQUIVw_def]
               THEN ONCE_REWRITE_TAC [MOD_ADD]
-              THEN ASM_SIMP_TAC arith_ss [MODw_IDEM2,MODw_2EXP_GT_WL]
+              THEN ASM_A_SIMP_TAC [MODw_IDEM2,MODw_2EXP_GT_WL]
          ]
     ]
 );
 
 val BITWISEw_WELLDEF = save_thm("BITWISEw_WELLDEF",SPEC `WL` BITWISE_WELLDEF);
 
-val OR_WELLDEF = REWRITE_RULE [GSYM OR_def] (SPEC `$\/` BITWISEw_WELLDEF);
+val OR_WELLDEF  = REWRITE_RULE [GSYM OR_def]  (SPEC `$\/` BITWISEw_WELLDEF);
 val AND_WELLDEF = REWRITE_RULE [GSYM AND_def] (SPEC `$/\` BITWISEw_WELLDEF);
 val EOR_WELLDEF = REWRITE_RULE [GSYM EOR_def] (SPEC `(\x y. ~(x = y))` BITWISEw_WELLDEF);
 
@@ -578,109 +575,70 @@ val EOR_WELLDEF = REWRITE_RULE [GSYM EOR_def] (SPEC `(\x y. ~(x = y))` BITWISEw_
 
 val SUC_WELLDEF = store_thm("SUC_WELLDEF",
   `!a b. a EQUIVw b ==> SUC a EQUIVw SUC b`,
-  RW_TAC std_ss [EQUIVw_def,ADD1]
+  B_RW_TAC [EQUIVw_def,ADD1]
     THEN ONCE_REWRITE_TAC [MOD_ADD]
     THEN ASM_REWRITE_TAC []
 );
 
 val ADD_WELLDEF = store_thm("ADD_WELLDEF",
   `!a b c d. a EQUIVw b /\ c EQUIVw d ==> a + c EQUIVw b + d`,
-  RW_TAC std_ss [EQUIVw_def]
+  B_RW_TAC [EQUIVw_def]
     THEN ONCE_REWRITE_TAC [MOD_ADD]
     THEN ASM_REWRITE_TAC []
 );
 
-val MUL_WELLDEF_LEM = store_thm("MUL_WELLDEF_LEM",
-  `!a b. (MODw a = 0) ==> (MODw (a * b) = 0)`,
-  Induct_on `b`
-    THENL [
-      RW_TAC std_ss [MODw_def,MULT_CLAUSES,ZERO_LT_TWOEXP,ZERO_MOD],
-      RW_TAC std_ss [MULT_CLAUSES]
-        THEN ONCE_REWRITE_TAC [MOD_ADD]
-        THEN FULL_SIMP_TAC std_ss []
-        THEN SIMP_TAC arith_ss [MODw_def,ZERO_LT_TWOEXP,ZERO_MOD]
-    ]
-);
-
-val MUL_WELLDEF_LEM2 = store_thm("MUL_WELLDEF_LEM2",
-  `!b. (MODw 0 = MODw b) ==> (MODw b = 0)`,
-  RW_TAC std_ss [MODw_def,ZERO_LT_TWOEXP,ZERO_MOD]
-);
 
 val MUL_WELLDEF = store_thm("MUL_WELLDEF",
   `!a b c d. a EQUIVw b /\ c EQUIVw d ==> a * c EQUIVw b * d`,
-  REWRITE_TAC [EQUIVw_def]
-    THEN Induct_on `a`
-    THEN REPEAT STRIP_TAC
-    THENL [
-      SIMP_TAC std_ss [MULT_CLAUSES]
-        THEN IMP_RES_TAC MUL_WELLDEF_LEM2
-        THEN ASM_SIMP_TAC std_ss [MUL_WELLDEF_LEM],
-      SIMP_TAC std_ss [MULT_CLAUSES]
-        THEN IMP_RES_TAC (REWRITE_RULE [EQUIVw_def] SUC_EQUIV_COMP)
-        THEN `MODw (a * c) = MODw ((b + (2 EXP WL - 1)) * d)` by PROVE_TAC []
-        THEN ONCE_REWRITE_TAC [MOD_ADD]
-        THEN ASM_SIMP_TAC std_ss []
-        THEN POP_ASSUM_LIST (K ALL_TAC)
-        THEN SIMP_TAC std_ss [RIGHT_ADD_DISTRIB,RIGHT_SUB_DISTRIB,MULT_CLAUSES,GSYM MOD_ADD]
-        THEN ONCE_REWRITE_TAC [GSYM ADD_ASSOC]
-        THEN SIMP_TAC std_ss [SUB_ADD,SIMP_RULE std_ss [exp_gteq,MULT_CLAUSES]
-                                                       (SPECL [`1`,`2 EXP WL`] LESS_MONO_MULT)]
-        THEN ONCE_REWRITE_TAC [ADD_COMM]
-        THEN ONCE_REWRITE_TAC [MULT_COMM]
-        THEN SIMP_TAC std_ss [MODw_def,ZERO_LT_TWOEXP,MOD_TIMES]
-    ]
-);
-
-(* MODw_MULT = |- !b a. MODw (a * b) = MODw (MODw a * MODw b) *)
-val MODw_MULT = save_thm("MODw_MULT",
-  GEN_ALL (SIMP_RULE std_ss [EQUIVw_def,MODw_IDEM2] (SPECL [`a`,`MODw a`,`b`,`MODw b`] MUL_WELLDEF))
+  B_RW_TAC [EQUIVw_def]
+    THEN ONCE_REWRITE_TAC [MODw_MULT]
+    THEN ASM_REWRITE_TAC []
 );
 
 val ONE_COMP_WELLDEF = store_thm("ONE_COMP_WELLDEF",
   `!a b. a EQUIVw b ==> ONE_COMP a EQUIVw ONE_COMP b`,
-  RW_TAC std_ss [EQUIVw_def,ONE_COMP_def]
+  B_RW_TAC [EQUIVw_def,ONE_COMP_def]
 );
 
 val TWO_COMP_WELLDEF = store_thm("TWO_COMP_WELLDEF",
   `!a b. a EQUIVw b ==> TWO_COMP a EQUIVw TWO_COMP b`,
-  RW_TAC std_ss [EQUIVw_def,TWO_COMP_def]
+  B_RW_TAC [EQUIVw_def,TWO_COMP_def]
 );
 
 val TOw_WELLDEF = store_thm("TOw_WELLDEF",
   `!a b. a EQUIVw b ==> MODw a EQUIVw MODw b`,
-  RW_TAC std_ss [EQUIVw_def]
+  B_RW_TAC [EQUIVw_def]
 );
 
 (* -------------------------------------------------------- *)
 
-val LSR_ONE_def = Define`LSR_ONE a = MODw a DIV 2`;
-val ASR_ONE_def = Define`ASR_ONE a = LSR_ONE a + SET (MSB a) HB`;
-val ROR_ONE_def = Define`ROR_ONE a = LSR_ONE a + SET (LSB a) HB`;
-val RRXn_def = Define`RRXn c a = LSR_ONE a + SET c HB`;
+val LSR_ONE_def = Define `LSR_ONE a = MODw a DIV 2`;
+val ASR_ONE_def = Define `ASR_ONE a = LSR_ONE a + SET (MSB a) HB`;
+val ROR_ONE_def = Define `ROR_ONE a = LSR_ONE a + SET (LSB a) HB`;
+val RRXn_def    = Define `RRXn c a  = LSR_ONE a + SET c HB`;
 
 val LSR_ONE_WELLDEF = store_thm("LSR_ONE_WELLDEF",
   `!a b. a EQUIVw b ==> LSR_ONE a EQUIVw LSR_ONE b`,
-  RW_TAC std_ss [EQUIVw_def,LSR_ONE_def]
+  B_RW_TAC [EQUIVw_def,LSR_ONE_def]
 );
 
 val ASR_ONE_WELLDEF = store_thm("ASR_ONE_WELLDEF",
   `!a b. a EQUIVw b ==> ASR_ONE a EQUIVw ASR_ONE b`,
-  RW_TAC std_ss [EQUIVw_def,ASR_ONE_def,LSR_ONE_def]
+  B_RW_TAC [EQUIVw_def,ASR_ONE_def,LSR_ONE_def]
     THEN IMP_RES_TAC (REWRITE_RULE [EQUIVw_def] MSB_WELLDEF)
-    THEN ASM_SIMP_TAC std_ss []
+    THEN ASM_REWRITE_TAC []
 );
 
 val ROR_ONE_WELLDEF = store_thm("ROR_ONE_WELLDEF",
   `!a b. a EQUIVw b ==> ROR_ONE a EQUIVw ROR_ONE b`,
-  RW_TAC std_ss [EQUIVw_def,ROR_ONE_def,LSR_ONE_def]
+  B_RW_TAC [EQUIVw_def,ROR_ONE_def,LSR_ONE_def]
     THEN IMP_RES_TAC (REWRITE_RULE [EQUIVw_def] LSB_WELLDEF)
-    THEN ASM_SIMP_TAC std_ss []
+    THEN ASM_REWRITE_TAC []
 );
 
 val RRX_WELLDEF = store_thm("RRX_WELLDEF",
   `!a b c. a EQUIVw b ==> (RRXn c) a EQUIVw (RRXn c) b`,
-  RW_TAC std_ss [EQUIVw_def,RRXn_def,LSR_ONE_def]
+  B_RW_TAC [EQUIVw_def,RRXn_def,LSR_ONE_def]
 );
 
 (* -------------------------------------------------------- *)
@@ -700,22 +658,23 @@ val LSR_ONE = store_thm("LSR_ONE",
 );
 
 (* -------------------------------------------------------- *)
-fun r(a,b,c,d) = {def_name=a,fixity=b,fname=c,func=d};
 
+fun r(a,b,c,d) = {def_name=a,fixity=b,fname=c,func=d};
+ 
 val [ADDw,ADD_0w,ADD1w,ADD_ASSOCw,ADD_CLAUSESw,
      ADD_COMMw,ADD_INV_0_EQw,EQ_ADD_LCANCELw,EQ_ADD_RCANCELw,
      LEFT_ADD_DISTRIBw,MULT_ASSOCw,MULT_COMMw,MULT_CLAUSESw,
      TOw_ELIM,ADD_TWO_COMP,TWO_COMP_ONE_COMP, OR_ASSOCw,OR_COMMw,
      OR_IDEMw,OR_ABSORBw,OR_COMPw,AND_ASSOCw,AND_COMMw,AND_IDEMw,
      AND_ABSORBw,AND_COMPw, ONE_COMPw,RIGHT_AND_OVER_ORw,RIGHT_OR_OVER_ANDw,
-     DE_MORGAN_THMw] 
- = 
+     DE_MORGAN_THMw]
+ =
  define_equivalence_type
    {name = "word",
     equiv = EQUIVw_QT,
     defs = [r("w_0_def",Prefix,"w_0",``0``),
             r("w_1_def",Prefix,"w_1",``AONE``),
-            r("w_T_def",Prefix,"w_T",``ATRUE``),
+            r("w_T_def",Prefix,"w_T",``COMP0``),
             r("SUCw_def",Prefix,"SUCw",``SUC``),
             r("ADDw_def",Infixl 500,"ADDw",``$+``),
             r("MULw_def",Infixl 550,"MULw",``$*``),
@@ -748,8 +707,9 @@ val [ADDw,ADD_0w,ADD1w,ADD_ASSOCw,ADD_CLAUSESw,
 val wn_def = Define `wn n = mk_word ($EQUIVw n)`;
 val NUMw_def = Define`NUMw w = MODw ($@ (dest_word w))`;
 
-val word_tybij = fetch "-" "word_tybij";
-val mk_word_one_one = BETA_RULE (prove_abs_fn_one_one (word_tybij));
+val word_tybij = definition "word_tybij";
+val mk_word_one_one  = BETA_RULE (prove_abs_fn_one_one word_tybij);
+val word_abs_fn_onto = BETA_RULE (prove_abs_fn_onto word_tybij);
 
 val _ = save_thm("ADDw",ADDw);
 val _ = save_thm("ADD_0w",ADD_0w);
@@ -777,38 +737,34 @@ val _ = save_thm("ONE_COMPw",ONE_COMPw);
 val _ = save_thm("RIGHT_AND_OVER_ORw",RIGHT_AND_OVER_ORw);
 val _ = save_thm("RIGHT_OR_OVER_ANDw",RIGHT_OR_OVER_ANDw);
 val _ = save_thm("DE_MORGAN_THMw",DE_MORGAN_THMw);
-val _ = save_thm("LEFT_AND_OVER_ORw",GEN_ALL (ONCE_REWRITE_RULE [AND_COMMw]
-                                             (SPECL [`b`,`c`,`a`] RIGHT_AND_OVER_ORw)));
-val _ = save_thm("LEFT_OR_OVER_ANDw",GEN_ALL (ONCE_REWRITE_RULE [OR_COMMw]
-                                             (SPECL [`b`,`c`,`a`] RIGHT_OR_OVER_ANDw)));
 
 val THE_WL = SIMP_RULE arithr_ss [HB_def,ADD1] WL_def;
  
 val w_0 = save_thm("w_0",REWRITE_RULE [GSYM wn_def] (definition "w_0_def"));
 val w_1 = save_thm("w_1",REWRITE_RULE [GSYM wn_def,AONE_def] (definition "w_1_def"));
-val w_T = save_thm("w_T",SIMP_RULE arithr_ss [GSYM wn_def,ATRUE_def,ONE_COMP_def,MODw_def,THE_WL] (definition "w_T_def"));
+val w_T = save_thm("w_T",SIMP_RULE arithr_ss [GSYM wn_def,COMP0_def,ONE_COMP_def,MODw_def,THE_WL] (definition "w_T_def"));
 
 val ADD_TWO_COMP = save_thm("ADD_TWO_COMP",REWRITE_RULE [TOw_ELIM] ADD_TWO_COMP);
 val ADD_TWO_COMP2 = save_thm("ADD_TWO_COMP2",ONCE_REWRITE_RULE [ADD_COMMw] ADD_TWO_COMP);
 
-val ADDw_def      = definition "ADDw_def";
-val MULw_def      = definition "MULw_def";
+val ADDw_def = definition "ADDw_def";
+val MULw_def = definition "MULw_def";
 val ONE_COMPw_def = definition "ONE_COMPw_def";
 val TWO_COMPw_def = definition "TWO_COMPw_def";
-val LSR_ONEw_def  = definition "LSR_ONEw_def";
-val ASR_ONEw_def  = definition "ASR_ONEw_def";
-val ROR_ONEw_def  = definition "ROR_ONEw_def";
-val RRXw_def      = definition "RRXw_def";
-val LSBw_def      = definition "LSBw_def";
-val MSBw_def      = definition "MSBw_def";
-val ORw_def       = definition "ORw_def";
-val ANDw_def      = definition "ANDw_def";
-val EORw_def      = definition "EORw_def";
+val LSR_ONEw_def = definition "LSR_ONEw_def";
+val ASR_ONEw_def = definition "ASR_ONEw_def";
+val ROR_ONEw_def = definition "ROR_ONEw_def";
+val RRXw_def = definition "RRXw_def";
+val LSBw_def = definition "LSBw_def";
+val MSBw_def = definition "MSBw_def";
+val ORw_def = definition "ORw_def";
+val ANDw_def = definition "ANDw_def";
+val EORw_def = definition "EORw_def";
 
 (* -------------------------------------------------------- *)
 
-val SUBw_def = 
-  new_infixl_definition 
+val SUBw_def =
+  new_infixl_definition
    ("SUBw_def",`a SUBw b = a ADDw (TWO_COMPw b)`,500);
 val LSLw_def = Define `LSLw n x = x MULw wn (2 EXP n)`;
 val LSRw_def = Define `LSRw n a = FUNPOW LSR_ONEw n a`;
@@ -824,7 +780,7 @@ val SLICEw_def = Define `SLICEw h l n = SLICE h l (NUMw n)`;
 val ssd = SIMPSET {ac = [(SPEC_ALL ADD_ASSOCw, SPEC_ALL ADD_COMMw)],
                 congs = [], convs = [], dprocs = [], filter = NONE, rewrs = []};
 
-val word_ss = std_ss++ssd;
+val word_ss = bool_ss++ssd;
 
 val TWO_COMP_ADD = store_thm("TWO_COMP_ADD",
   `!a b. TWO_COMPw (a ADDw b) = TWO_COMPw a ADDw TWO_COMPw b`,
@@ -836,7 +792,7 @@ val TWO_COMP_ADD = store_thm("TWO_COMP_ADD",
        by REWRITE_TAC [ADD_TWO_COMP2,ADD_CLAUSESw]
      THEN RULE_ASSUM_TAC (REWRITE_RULE [rearrange])
      THEN ASSUME_TAC (SYM (SPEC `a ADDw b` ADD_TWO_COMP2))
-     THEN FULL_SIMP_TAC std_ss [EQ_ADD_RCANCELw]
+     THEN B_FULL_SIMP_TAC [EQ_ADD_RCANCELw]
   end
 );
 
@@ -860,12 +816,12 @@ val ADD_SUB_SYM = store_thm("ADD_SUB_SYM",
 
 val SUB_EQUALw = store_thm("SUB_EQUALw",
   `!a. a SUBw a = w_0`,
-   RW_TAC std_ss [SUBw_def,ADD_TWO_COMP]
+   B_RW_TAC [SUBw_def,ADD_TWO_COMP]
 );
 
 val ADD_SUBw = store_thm("ADD_SUBw",
   `!a b. a ADDw b SUBw b = a`,
-  RW_TAC std_ss [ADD_SUB_ASSOC,SUB_EQUALw,ADD_0w]
+  B_RW_TAC [ADD_SUB_ASSOC,SUB_EQUALw,ADD_0w]
 );
 
 val SUB_ADDw = REWRITE_RULE [ADD_SUB_SYM] ADD_SUBw;
@@ -877,25 +833,25 @@ val SUB_SUBw = store_thm("SUB_SUBw",
 
 val ONE_COMP_TWO_COMP = store_thm("ONE_COMP_TWO_COMP",
   `!a. ONE_COMPw a = TWO_COMPw a SUBw w_1`,
-  RW_TAC std_ss [TWO_COMP_ONE_COMP,ADD_SUBw]
+  B_RW_TAC [TWO_COMP_ONE_COMP,ADD_SUBw]
 );
 
 val SUBw = store_thm("SUBw",
   `!m n. SUCw m SUBw n = SUCw (m SUBw n)`,
-  RW_TAC std_ss [ADD1w,ADD_SUB_SYM]
+  B_RW_TAC [ADD1w,ADD_SUB_SYM]
 );
 
 val ADD_EQ_SUBw = store_thm("ADD_EQ_SUBw",
   `!m n p. (m ADDw n = p) = (m = p SUBw n)`,
   REPEAT STRIP_TAC THEN EQ_TAC
-    THEN RW_TAC std_ss [SUB_ADDw]
+    THEN B_RW_TAC [SUB_ADDw]
     THEN REWRITE_TAC [ADD_SUBw]
 );
 
 val CANCEL_SUBw = store_thm("CANCEL_SUBw",
   `!m n p. (n SUBw p = m SUBw p) = (n = m)`,
   REPEAT STRIP_TAC THEN EQ_TAC
-    THEN RW_TAC std_ss [GSYM ADD_EQ_SUBw,ADD_SUBw,SUB_ADDw]
+    THEN B_RW_TAC [GSYM ADD_EQ_SUBw,ADD_SUBw,SUB_ADDw]
 );
 
 val SUB_PLUSw = store_thm("SUB_PLUSw",
@@ -905,13 +861,19 @@ val SUB_PLUSw = store_thm("SUB_PLUSw",
 
 (* -------------------------------------------------------- *)
  
+val word_nchotomy = store_thm("word_nchotomy",
+  `!w. ?n. w = wn n`,
+  PROVE_TAC [wn_def,word_abs_fn_onto]
+);
+
 val EQUIV_EXISTS = prove(`!y. ?x. $EQUIVw y = $EQUIVw x`, PROVE_TAC []);
 
-val mk_word_eq_one_one = SIMP_RULE std_ss [EQUIV_EXISTS] (SPECL [`$EQUIVw x`,`$EQUIVw y`] mk_word_one_one);
+(* |- (mk_word ($EQUIVw x) = mk_word ($EQUIVw y)) = ($EQUIVw x = $EQUIVw y) *)
+val mk_word_eq_one_one = SIMP_RULE bool_ss [EQUIV_EXISTS] (SPECL [`$EQUIVw x`,`$EQUIVw y`] mk_word_one_one);
 
 val dest_word_mk_word_eq = prove(
   `!a. dest_word (mk_word ($EQUIVw a)) = $EQUIVw a`,
-  STRIP_TAC THEN SIMP_TAC std_ss [EQUIV_EXISTS,GSYM (BETA_RULE word_tybij)]
+  STRIP_TAC THEN REWRITE_TAC [EQUIV_EXISTS,GSYM (BETA_RULE word_tybij)]
 );
 
 val dest_word_mk_word_eq2 = prove(
@@ -921,209 +883,416 @@ val dest_word_mk_word_eq2 = prove(
 
 (* |- !a. dest_word (mk_word (EQUIVw a)) = EQUIVw a *)
 val dest_word_mk_word_eq3 = save_thm("dest_word_mk_word_eq3",
-  GEN_ALL (REWRITE_RULE [GSYM FUN_EQ_THM] (GEN `x` (SPEC_ALL dest_word_mk_word_eq2)))
+  (GEN_ALL o REWRITE_RULE [GSYM FUN_EQ_THM] o GEN `x` o SPEC_ALL) dest_word_mk_word_eq2
 );
 
 val dest_word_mk_word_exists = prove(
   `?x. dest_word (mk_word ($EQUIVw a)) x`,
-  RW_TAC std_ss [dest_word_mk_word_eq2,EQUIVw_def] THEN PROVE_TAC []
-);
-
-val SELECT_WORD_TAC =
-    `!p:num -> bool. $@p = @x. p x` by
-              (GEN_TAC THEN CONV_TAC (ONCE_DEPTH_CONV ETA_CONV) THEN PROVE_TAC [])
-    THEN POP_ASSUM (fn th => ONCE_REWRITE_TAC [th]) THEN SELECT_TAC
-    THEN RW_TAC std_ss [dest_word_mk_word_exists,dest_word_mk_word_eq2];
-
-val NUMw_EVAL = store_thm("NUMw_EVAL",
-  `!n. NUMw (wn n) = MODw n`,
-  RW_TAC std_ss [NUMw_def,wn_def]
-    THEN SELECT_WORD_TAC
-    THEN FULL_SIMP_TAC std_ss [EQUIVw_def]
+  B_RW_TAC [dest_word_mk_word_eq2,EQUIVw_def] THEN PROVE_TAC []
 );
 
 (* -------------------------------------------------------- *)
  
+val etar = prove(
+  `!p:num -> bool. $@p = @x. p x`,
+  GEN_TAC THEN CONV_TAC (ONCE_DEPTH_CONV ETA_CONV) THEN PROVE_TAC []
+);
+
 val MODw_ELIM = store_thm("MODw_ELIM",
   `!n. wn (MODw n) = wn n`,
-  RW_TAC std_ss [wn_def,mk_word_eq_one_one]
+  B_RW_TAC [wn_def,mk_word_eq_one_one]
     THEN ONCE_REWRITE_TAC [FUN_EQ_THM]
     THEN REWRITE_TAC [EQUIVw_def,MODw_IDEM2]
 );
 
+val NUMw_EVAL = store_thm("NUMw_EVAL",
+  `!n. NUMw (wn n) = MODw n`,
+  B_RW_TAC [NUMw_def,wn_def]
+    THEN ONCE_REWRITE_TAC [etar] THEN SELECT_TAC
+    THEN B_RW_TAC [dest_word_mk_word_exists,dest_word_mk_word_eq2]
+    THEN B_FULL_SIMP_TAC [EQUIVw_def]
+);
+
+(* -------------------------------------------------------- *)
+ 
+fun SELECT_WORD_TAC th1 th2 =
+  B_SIMP_TAC [wn_def,th1,mk_word_eq_one_one]
+    THEN ONCE_REWRITE_TAC [etar] THEN SELECT_TAC
+    THEN B_RW_TAC [dest_word_mk_word_exists,dest_word_mk_word_eq2]
+    THEN ASM_B_SIMP_TAC [th2,EQUIVw_SYM,GSYM EQUIVw_QT];
+
 val ADD_EVAL = store_thm("ADD_EVAL",
   `(wn a) ADDw (wn b) = wn (a + b)`,
-  SIMP_TAC std_ss [wn_def,ADDw_def,mk_word_eq_one_one]
-    THEN SELECT_WORD_TAC
-    THEN REWRITE_TAC [GSYM EQUIVw_QT]
-    THEN `a + b EQUIVw x + x'` by IMP_RES_TAC ADD_WELLDEF
-    THEN ASM_SIMP_TAC std_ss [EQUIVw_SYM]
-);
+  SELECT_WORD_TAC ADDw_def ADD_WELLDEF);
 
 val MUL_EVAL = store_thm("MUL_EVAL",
   `(wn a) MULw (wn b) = wn (a * b)`,
-  SIMP_TAC std_ss [wn_def,MULw_def,mk_word_eq_one_one]
-    THEN SELECT_WORD_TAC
-    THEN REWRITE_TAC [GSYM EQUIVw_QT]
-    THEN `a * b EQUIVw x * x'` by IMP_RES_TAC MUL_WELLDEF
-    THEN ASM_SIMP_TAC std_ss [EQUIVw_SYM]
-);
+  SELECT_WORD_TAC MULw_def MUL_WELLDEF);
 
 val ONE_COMP_EVAL = store_thm("ONE_COMP_EVAL",
   `ONE_COMPw (wn a) = wn (ONE_COMP a)`,
-  SIMP_TAC std_ss [wn_def,ONE_COMPw_def,mk_word_eq_one_one]
-    THEN SELECT_WORD_TAC
-    THEN ONCE_REWRITE_TAC [FUN_EQ_THM]
-    THEN FULL_SIMP_TAC std_ss [EQUIVw_def,ONE_COMP_def]
-);
+  SELECT_WORD_TAC ONE_COMPw_def ONE_COMP_WELLDEF);
 
 val TWO_COMP_EVAL = store_thm("TWO_COMP_EVAL",
   `TWO_COMPw (wn a) = wn (TWO_COMP a)`,
-  SIMP_TAC std_ss [wn_def,TWO_COMPw_def,mk_word_eq_one_one]
-    THEN SELECT_WORD_TAC
-    THEN ONCE_REWRITE_TAC [FUN_EQ_THM]
-    THEN FULL_SIMP_TAC std_ss [EQUIVw_def,TWO_COMP_def]
-);
+  SELECT_WORD_TAC TWO_COMPw_def TWO_COMP_WELLDEF);
 
 val LSR_ONE_EVAL = store_thm("LSR_ONE_EVAL",
   `LSR_ONEw (wn a) = wn (LSR_ONE a)`,
-  SIMP_TAC std_ss [wn_def,LSR_ONEw_def,LSR_ONE_def,mk_word_eq_one_one]
-    THEN SELECT_WORD_TAC
-    THEN REWRITE_TAC [GSYM EQUIVw_QT]
-    THEN IMP_RES_TAC LSR_ONE_WELLDEF
-    THEN FULL_SIMP_TAC std_ss [LSR_ONE_def,EQUIVw_SYM]
-);
+  SELECT_WORD_TAC LSR_ONEw_def LSR_ONE_WELLDEF);
 
 val ASR_ONE_EVAL = store_thm("ASR_ONE_EVAL",
   `ASR_ONEw (wn a) = wn (ASR_ONE a)`,
-  SIMP_TAC std_ss [wn_def,ASR_ONEw_def,mk_word_eq_one_one]
-    THEN SELECT_WORD_TAC
-    THEN REWRITE_TAC [GSYM EQUIVw_QT]
-    THEN IMP_RES_TAC ASR_ONE_WELLDEF
-    THEN FULL_SIMP_TAC std_ss [EQUIVw_SYM]
+  SELECT_WORD_TAC ASR_ONEw_def ASR_ONE_WELLDEF
 );
 
 val ROR_ONE_EVAL = store_thm("ROR_ONE_EVAL",
   `ROR_ONEw (wn a) = wn (ROR_ONE a)`,
-  SIMP_TAC std_ss [wn_def,ROR_ONEw_def,mk_word_eq_one_one]
-    THEN SELECT_WORD_TAC
-    THEN REWRITE_TAC [GSYM EQUIVw_QT]
-    THEN IMP_RES_TAC ROR_ONE_WELLDEF
-    THEN FULL_SIMP_TAC std_ss [EQUIVw_SYM]
+  SELECT_WORD_TAC ROR_ONEw_def ROR_ONE_WELLDEF
 );
 
 val RRX_EVAL = store_thm("RRX_EVAL",
   `RRXw c (wn a) = wn (RRXn c a)`,
-  SIMP_TAC std_ss [wn_def,RRXw_def,mk_word_eq_one_one]
-    THEN SELECT_WORD_TAC
-    THEN REWRITE_TAC [GSYM EQUIVw_QT]
-    THEN IMP_RES_TAC RRX_WELLDEF
-    THEN FULL_SIMP_TAC std_ss [EQUIVw_SYM]
+  SELECT_WORD_TAC RRXw_def RRX_WELLDEF
 );
 
 val LSB_EVAL = store_thm("LSB_EVAL",
   `LSBw (wn a) = LSB a`,
-  SIMP_TAC std_ss [wn_def,LSBw_def]
-    THEN SELECT_WORD_TAC
-    THEN REWRITE_TAC [GSYM EQUIVw_QT]
-    THEN IMP_RES_TAC LSB_WELLDEF
-    THEN FULL_SIMP_TAC std_ss [EQUIVw_SYM]
+  SELECT_WORD_TAC LSBw_def LSB_WELLDEF
 );
 
 val MSB_EVAL = store_thm("MSB_EVAL",
   `MSBw (wn a) = MSB a`,
-  SIMP_TAC std_ss [wn_def,MSBw_def]
-    THEN SELECT_WORD_TAC
-    THEN REWRITE_TAC [GSYM EQUIVw_QT]
-    THEN IMP_RES_TAC MSB_WELLDEF
-    THEN FULL_SIMP_TAC std_ss [EQUIVw_SYM]
+  SELECT_WORD_TAC MSBw_def MSB_WELLDEF
 );
 
 val OR_EVAL = store_thm("OR_EVAL",
   `(wn a) ORw (wn b) = wn (OR a b)`,
-  SIMP_TAC std_ss [wn_def,ORw_def,mk_word_eq_one_one]
-    THEN SELECT_WORD_TAC
-    THEN REWRITE_TAC [GSYM EQUIVw_QT]
-    THEN IMP_RES_TAC OR_WELLDEF
-    THEN FULL_SIMP_TAC std_ss [EQUIVw_SYM]
+  SELECT_WORD_TAC ORw_def OR_WELLDEF
 );
 
 val EOR_EVAL = store_thm("EOR_EVAL",
   `(wn a) EORw (wn b) = wn (EOR a b)`,
-  SIMP_TAC std_ss [wn_def,EORw_def,mk_word_eq_one_one]
-    THEN SELECT_WORD_TAC
-    THEN REWRITE_TAC [GSYM EQUIVw_QT]
-    THEN IMP_RES_TAC EOR_WELLDEF
-    THEN FULL_SIMP_TAC std_ss [EQUIVw_SYM]
+  SELECT_WORD_TAC EORw_def EOR_WELLDEF
 );
 
 val AND_EVAL = store_thm("AND_EVAL",
   `(wn a) ANDw (wn b) = wn (AND a b)`,
-  SIMP_TAC std_ss [wn_def,ANDw_def,mk_word_eq_one_one]
-    THEN SELECT_WORD_TAC
-    THEN REWRITE_TAC [GSYM EQUIVw_QT]
-    THEN IMP_RES_TAC AND_WELLDEF
-    THEN FULL_SIMP_TAC std_ss [EQUIVw_SYM]
+  SELECT_WORD_TAC ANDw_def AND_WELLDEF
 );
 
 val BITS_EVAL = store_thm("BITS_EVAL",
   `!h l a. BITSw h l (wn a) = BITS h l (MODw a)`,
-  RW_TAC std_ss [BITSw_def,NUMw_EVAL]
+  B_RW_TAC [BITSw_def,NUMw_EVAL]
 );
 
 val BIT_EVAL = store_thm("BIT_EVAL",
   `!b a. BITw b (wn a) = BIT b (MODw a)`,
-  RW_TAC std_ss [BITw_def,NUMw_EVAL]
+  B_RW_TAC [BITw_def,NUMw_EVAL]
 );
 
 val SLICE_EVAL = store_thm("SLICE_EVAL",
   `!h l a. SLICEw h l (wn a) = SLICE h l (MODw a)`,
-  RW_TAC std_ss [SLICEw_def,NUMw_EVAL]
+  B_RW_TAC [SLICEw_def,NUMw_EVAL]
 );
 
 (* -------------------------------------------------------- *)
 
 val MOD_MOD_DIV = store_thm("MOD_MOD_DIV",
-  `!a b. 0 < b ==> INw (MODw a DIV b)`,
-  REPEAT STRIP_TAC
-    THEN Cases_on `b = 1`
-    THENL [
-      ASM_SIMP_TAC std_ss [DIV1,INw_MODw],
-      REWRITE_TAC [MODw_def]
-        THEN Cases_on `a MOD 2 EXP WL = 0`
-        THENL [
-          ASM_SIMP_TAC arith_ss [ZERO_DIV,ZERO_LT_TWOEXP,INw_def],
-          RULE_ASSUM_TAC (REWRITE_RULE [NOT_ZERO_LT_ZERO])
-            THEN `1 < b` by DECIDE_TAC
-            THEN IMP_RES_TAC DIV_LESS
-            THEN ASSUME_TAC (SPEC `a` MODw_LESS)
-            THEN `a MOD 2 EXP WL DIV b < 2 EXP WL` by IMP_RES_TAC LESS_TRANS
-            THEN ASM_SIMP_TAC std_ss [INw_def]
-        ]
-    ]
+  `!a b. INw (MODw a DIV 2 EXP b)`,
+  A_RW_TAC [MODw_THM,BITS_DIV_THM]
+    THEN ASSUME_TAC (SPECL [`HB`,`b`,`a`] BITSLT_THM)
+    THEN ASSUME_TAC (SPECL [`SUC HB`,`b`] EXP_SUB_LESS_EQ)
+    THEN IMP_RES_TAC LESS_LESS_EQ_TRANS
+    THEN ASM_REWRITE_TAC [WL_def,INw_def]
 );
 
 val MOD_MOD_DIV_2EXP = store_thm("MOD_MOD_DIV_2EXP",
   `!a n. MODw (MODw a DIV 2 EXP n) DIV 2 = MODw a DIV 2 EXP SUC n`,
-   REPEAT STRIP_TAC
-     THEN ASSUME_TAC (SIMP_RULE arith_ss [ZERO_LT_TWOEXP] (SPECL [`a`,`2 EXP n`] MOD_MOD_DIV))
-     THEN ASM_SIMP_TAC arith_ss [ZERO_LT_TWOEXP,DIV_DIV_DIV_MULT,TOw_IDEM,
-                             GSYM (ONCE_REWRITE_RULE [MULT_COMM] EXP)]
+  A_RW_TAC [ZERO_LT_TWOEXP,DIV_DIV_DIV_MULT,TOw_IDEM,MOD_MOD_DIV,
+            GSYM (ONCE_REWRITE_RULE [MULT_COMM] EXP)]
 );
 
 val LSR_EVAL = store_thm("LSR_EVAL",
   `!n. LSRw n (wn a) = wn (MODw a DIV 2 EXP n)`,
   Induct_on `n`
     THENL [
-       SIMP_TAC std_ss [FUNPOW,LSRw_def,EXP,DIV1,MODw_ELIM],
-       FULL_SIMP_TAC std_ss [LSRw_def,FUNPOW_THM2,LSR_ONE_EVAL,LSR_ONE_def,MOD_MOD_DIV_2EXP]
+       B_SIMP_TAC [FUNPOW,LSRw_def,EXP,DIV1,MODw_ELIM],
+       B_FULL_SIMP_TAC [LSRw_def,FUNPOW_THM2,LSR_ONE_EVAL,LSR_ONE_def,MOD_MOD_DIV_2EXP]
     ]
 );
 
+val LSR_MIN_THM = store_thm("LSR_MIN_THM",
+  `!a n.  LSRw n a = FUNPOW LSR_ONEw (MIN n WL) a`,
+  REPEAT STRIP_TAC
+    THEN REWRITE_TAC [GSYM LSRw_def]
+    THEN STRUCT_CASES_TAC (SPEC `a` word_nchotomy)
+    THEN B_RW_TAC [LSR_EVAL,MIN_DEF]
+    THEN RULE_ASSUM_TAC (REWRITE_RULE [NOT_LESS])
+    THEN IMP_RES_TAC LESS_EQUAL_ADD
+    THEN A_RW_TAC [REWRITE_RULE [INw_def] INw_MODw,LESS_DIV_EQ_ZERO,
+                   GSYM DIV_DIV_DIV_MULT,EXP_ADD,ZERO_LT_TWOEXP]
+);
+
+(* -------------------------------------------------------- *)
+
+val MOD_WL = (GEN_ALL o CONJUNCT2 o SPEC_ALL o REWRITE_RULE [WL_POS] o SPEC `WL`) DIVISION;
+
+val wn_TIMES = prove(
+  `!a b. wn (a * 2 EXP WL + b) = wn b`,
+  ONCE_REWRITE_TAC [GSYM MODw_ELIM]
+    THEN B_SIMP_TAC [MODw_def,MOD_TIMES,ZERO_LT_TWOEXP]
+);
+
+val wn_TIMES2 = ONCE_REWRITE_RULE [ADD_COMM] wn_TIMES;
+
+val LEFT_SHIFT_LESS = store_thm("LEFT_SHIFT_LESS",
+  `!n m a. a < 2 EXP m ==> 2 EXP n + a * 2 EXP n <= 2 EXP (m + n)`,
+  A_RW_TAC [GSYM MULT,LESS_EQ,EXP_ADD,LESS_MONO_MULT]
+);
+
+val lem = prove(
+  `!a b c d. a < b /\ b + c <= d ==> a + c < d`,
+  A_RW_TAC []
+);
+
+val lem2 = prove(
+  `!a b m n. a < 2 EXP n /\ b < 2 EXP m ==> a + b * 2 EXP n < 2 EXP (m + n)`,
+  PROVE_TAC [LEFT_SHIFT_LESS,lem]
+);
+
+val lem3 = prove(
+  `!a b h l. l <= h /\ a < 2 EXP (h - l) /\ b < 2 EXP l ==> a + b * 2 EXP (h - l) < 2 EXP h`,
+  REPEAT STRIP_TAC
+    THEN `a + b * 2 EXP (h - l) < 2 EXP (l + (h - l))` by IMP_RES_TAC (SPECL [`a`,`b`,`l`,`h - l`] lem2)
+    THEN PAT_ASSUM `l <= h` (fn th => RULE_ASSUM_TAC (SIMP_RULE arith_ss [th,GSYM LESS_EQ_ADD_SUB]))
+    THEN A_FULL_SIMP_TAC []
+);
+
+val lem4 = prove(
+  `!x n. 0 < x MOD WL ==> INw (BITS HB (x MOD WL) n + BITS (x MOD WL - 1) 0 n * 2 EXP (WL - x MOD WL))`,
+  B_RW_TAC [INw_def]
+    THEN RULE_ASSUM_TAC (REWRITE_RULE [GSYM ONE,LESS_EQ])
+    THEN POP_ASSUM (fn th =>
+           ASSUME_TAC (SIMP_RULE arith_ss [th,ADD1,SUB_ADD] (SPECL [`x MOD WL - 1`,`0`,`n`] BITSLT_THM)))
+    THEN ASSUME_TAC (REWRITE_RULE [GSYM WL_def] (SPECL [`HB`,`x MOD WL`,`n`] BITSLT_THM))
+    THEN ASSUME_TAC (MATCH_MP LESS_IMP_LESS_OR_EQ (SPEC `x` MOD_WL))
+    THEN ASM_B_SIMP_TAC [lem3]
+);
+
+val lem5 = prove(
+  `!x n. MODw (BITS HB (x MOD WL) n + BITS (x MOD WL - 1) 0 n * 2 EXP (WL - x MOD WL)) =
+          if x MOD WL = 0 then BITS HB 0 n
+                          else BITS HB (x MOD WL) n + BITS (x MOD WL - 1) 0 n * 2 EXP (WL - x MOD WL)`,
+  B_RW_TAC []
+    THENL [
+       A_SIMP_TAC [MOD_TIMES,ZERO_LT_TWOEXP,MOD_MOD,MODw_def,GSYM MODw_THM],
+       RULE_ASSUM_TAC (REWRITE_RULE [NOT_ZERO_LT_ZERO])
+         THEN ASM_B_SIMP_TAC [lem4,TOw_IDEM]
+    ]
+);
+
+val lem6 = prove(
+  `!h b n. (BITS b b n MOD 2 = 1) = BIT b n`,
+  A_RW_TAC [GSYM ODD_MOD2_LEM,GSYM LSB_ODD,LSB_def,BIT_def,BITS_COMP_THM]
+);
+
+val lem7 = PROVE [MULT_COMM,MULT_ASSOC] `!a b c. a * (b * c) = (a * c) * b`;
+
+(* |- !n l h. BITS h l n DIV 2 = BITS h (l + 1) n *)
+val BITS_DIV_THM2 = (REWRITE_RULE [EXP_1] o GEN_ALL o INST [`n` |-> `1`] o SPEC_ALL) BITS_DIV_THM;
+
+(* |- !n. BITS 0 0 n = n MOD 2 *)
+val BITS00 = GEN_ALL (REWRITE_CONV [SUC_SUB,DIV1,EXP,EXP_1,SYM TWO,BITS_THM] ``BITS 0 0 n``);
+
+val SPEC_MOD_PLUS_1 = REWRITE_RULE [WL_POS] (SPEC `WL` MOD_PLUS_1);
+val SPEC_MOD_ADD_1  = REWRITE_RULE [WL_POS] (SPEC `WL` MOD_ADD_1);
+
+(* |- !n x. RORw (SUC x) n = ROR_ONEw (RORw x n) *)
+val ROR_LEM = GEN_ALL (RIGHT_REWRITE_RULE [GSYM RORw_def]
+                 (SIMP_CONV bool_ss [RORw_def,FUNPOW_THM2] ``RORw (SUC x) n``));
+
+val ROR_THM = store_thm("ROR_THM",
+  `!x n. RORw x (wn n) = let x' = x MOD WL in
+                          wn (BITS HB x' n + (BITS (x' - 1) 0 n) * 2 EXP (WL - x'))`,
+  Induct_on `x`
+    THEN REPEAT STRIP_TAC
+    THENL [
+      A_SIMP_TAC [ZERO_MOD,WL_POS,RORw_def,FUNPOW,wn_TIMES2,SYM MODw_THM,MODw_ELIM],
+      POP_ASSUM (fn th => S_SIMP_TAC [th,ROR_LEM,ROR_ONE_EVAL,ROR_ONE_def,LSR_ONE_def])
+        THEN Cases_on `(x + 1) MOD WL = 0`
+        THENL [
+           IMP_RES_TAC SPEC_MOD_PLUS_1
+             THEN RULE_ASSUM_TAC (SIMP_RULE bool_ss [ADD_EQ_SUB,WL_GEQ_ONE,WL_SUB_ONE])
+             THEN R_RW_TAC [lem5,lem6,ADD1,WL_SUB_HB,EXP_1,wn_TIMES,wn_TIMES2,MODw_THM,
+                            MODw_ELIM,ADD_DIV_ADD_DIV,BITS_DIV_THM2,BITS_ZERO,
+                            LSB_ODD,ODD_MOD2_LEM,MOD_TIMES]
+             THENL [
+               R_RW_TAC [SET_def,BIT_def] THEN B_FULL_SIMP_TAC [NOT_BITS2],
+               IMP_RES_TAC NOT_ZERO_ADD1
+                 THEN ASM_B_SIMP_TAC [SUC_SUB1,SIMP_RULE arith_ss [] (SPECL [`p`,`0`] BITS_SUC)]
+             ],
+           IMP_RES_TAC SPEC_MOD_ADD_1
+             THEN A_RW_TAC [ADD1,BITS_DIV_THM2,WL_SUB_ONE,lem5]
+             THENL [
+               R_SIMP_TAC [lem7,WL_def,LSB_ODD,ODD_MOD2_LEM,EXP,MOD_TIMES]
+                 THEN A_SIMP_TAC [GSYM BITS00,BITS_COMP_THM,GSYM BIT_def,SLICE_COR,
+                                  REWRITE_RULE [ADD] (SPECL [`HB`,`0`] BIT_SLICE_LEM)],
+               IMP_RES_TAC NOT_ZERO_ADD1 THEN POP_ASSUM (K ALL_TAC)
+                 THEN POP_ASSUM (fn th => SIMP_TAC bool_ss [th,SUC_SUB1,WL_SUB_SUC_X,SUB_PLUS] THEN
+                          ASSUME_TAC (REWRITE_RULE [th,WL_def,ADD1,LESS_MONO_ADD_EQ] (SPEC `x` MOD_WL)))
+                 THEN IMP_RES_TAC LESS_ADD_1
+                 THEN RULE_ASSUM_TAC (ONCE_REWRITE_RULE [ADD_COMM])
+                 THEN ASM_A_SIMP_TAC [LSB_ODD,ODD_MOD2_LEM,GSYM ADD1,EXP,MOD_TIMES,
+                                      lem7,BITS_DIV_THM2,ADD_DIV_ADD_DIV]
+                 THEN A_SIMP_TAC [GSYM BITS00,BITS_COMP_THM,GSYM BIT_def,BIT_SLICE_LEM]
+                 THEN B_SIMP_TAC [DECIDE (Term `a + SUC b = SUC a + b`),
+                                  BIT_SLICE_LEM,ADD_ASSOC,GSYM RIGHT_ADD_DISTRIB,GSYM SLICE_COR]
+                 THEN A_SIMP_TAC [ONCE_REWRITE_RULE [ADD_COMM] SLICE_COMP_THM]
+             ]
+        ]
+    ]
+);
+
+(* -------------------------------------------------------- *)
+
+val lem = prove(
+  `!x n. ~MSB n ==> ~MSB (BITS HB x n)`,
+  A_RW_TAC [MSB_def,BIT_def,MIN_DEF,BITS_COMP_THM2,BITS_ZERO]
+    THEN `x = 0` by DECIDE_TAC
+    THEN ASM_REWRITE_TAC [ADD]
+);
+
+val lem2 = prove(
+  `!h l n. LSR_ONE (BITS HB l n) = BITS HB (SUC l) n`,
+  A_RW_TAC [MIN_DEF,LSR_ONE,ADD1,BITS_COMP_THM2]
+    THEN Cases_on `l = 0`
+    THEN A_FULL_SIMP_TAC []
+);
+
+val lem3 = prove(
+  `!n. ~MSB n ==> (BITS HB HB n = 0)`,
+  B_RW_TAC [BIT_def,MSB_def,NOT_BITS2]
+);
+
+val lem4 = prove(
+  `!n. MSB n ==> (BITS HB HB n = 1)`,
+  B_RW_TAC [MSB_def,BIT_def]
+);
+
+val lem5 = prove(
+  `!a b c. c < a /\ c < b ==> a - b + c < a`,
+  A_RW_TAC [SUB_RIGHT_ADD]
+);
+
+val lem6 = prove(
+  `!h x n. 2 EXP SUC h - 2 EXP (SUC h - x) + BITS h x n < 2 EXP SUC h`,
+  REPEAT STRIP_TAC
+    THEN ASSUME_TAC (SPECL [`h`,`x`,`n`] BITSLT_THM)
+    THEN ASSUME_TAC (SPECL [`SUC h`,`x`] EXP_SUB_LESS_EQ)
+    THEN IMP_RES_TAC LESS_LESS_EQ_TRANS
+    THEN ASM_B_SIMP_TAC [lem5]
+);
+
+(* |- !x n. 2 EXP WL - 2 EXP (WL - x) + BITS HB x n < 2 EXP WL *)
+val lem6b = REWRITE_RULE [GSYM WL_def] (SPEC `HB` lem6);
+
+val lem6c = prove(
+  `!h x n. 2 EXP h - 2 EXP (h - x) + BITS h (SUC x) n < 2 EXP h`,
+  REPEAT STRIP_TAC
+    THEN ASSUME_TAC (SIMP_RULE arith_ss [] (SPECL [`h`,`SUC x`,`n`] BITSLT_THM))
+    THEN ASSUME_TAC (SPECL [`h`,`x`] EXP_SUB_LESS_EQ)
+    THEN IMP_RES_TAC LESS_LESS_EQ_TRANS
+    THEN ASM_B_SIMP_TAC [lem5]
+);
+
+val lem7 = prove(
+  `!x n. LSR_ONE (2 EXP WL - 2 EXP (WL - x) + BITS HB x n) =
+           (2 EXP WL - 2 EXP (WL - x) + BITS HB x n) DIV 2`,
+  B_RW_TAC [LSR_ONE_def,MODw_THM,EXP,DIV1,REWRITE_RULE [GSYM WL_def] (SPEC `HB` BITS_LT_HIGH),lem6b]
+);
+
+val lem8 = prove(
+  `!h x. x <= h ==> (2 EXP SUC h - 2 EXP (SUC h - x) = (2 EXP h - 2 EXP (h - x)) * 2)`,
+  B_RW_TAC [ADD1,ONCE_REWRITE_RULE [ADD_COMM] LESS_EQ_ADD_SUB]
+    THEN A_SIMP_TAC [GSYM ADD1,EXP,RIGHT_SUB_DISTRIB]
+);
+
+(* |- !x.  x <= HB ==> (2 EXP WL - 2 EXP (WL - x) = (2 EXP HB - 2 EXP (HB - x)) * 2) *)
+val lem8b = REWRITE_RULE [GSYM WL_def] (SPEC `HB` lem8);
+
+val lem8c = prove(
+  `!x n. x <= HB ==> ((2 EXP WL - 2 EXP (WL - x) + BITS HB x n) DIV 2 =
+                       2 EXP HB - 2 EXP (HB - x) + BITS HB (SUC x) n)`,
+  A_RW_TAC [lem8b,ADD_DIV_ADD_DIV,ZERO_LT_TWOEXP,REWRITE_RULE [GSYM ADD1] BITS_DIV_THM2]
+);
+
+val lem9 = prove(
+  `!x n. x <= HB /\ MSB n ==> MSB (2 EXP WL - 2 EXP (WL - x) + BITS HB x n)`,
+  B_RW_TAC [MSB_def,BIT_def,REWRITE_RULE [GSYM WL_def] (SPEC `HB` BITS_LT_HIGH),lem6b]
+    THEN Cases_on `x = 0`
+    THENL [
+       ASM_A_SIMP_TAC [BITS_THM,CONJUNCT1 EXP,DIV1]
+         THEN ASM_REWRITE_TAC [GSYM BITS2_THM],
+       IMP_RES_TAC NOT_ZERO_ADD1
+         THEN ASM_A_SIMP_TAC [EXP,WL_def]
+         THEN B_SIMP_TAC [LESS_EQ_ADD_SUB,EXP_SUB_LESS_EQ,lem6c,TIMES2,GSYM ADD_ASSOC,DIV_MULT_1]
+    ]
+);
+
+val lem10 = prove(
+  `!a b. 2 EXP a <= 2 EXP (a - b) ==> (a = 0) \/ (b = 0)`,
+  REPEAT STRIP_TAC
+    THEN ASSUME_TAC (SPEC_ALL EXP_SUB_LESS_EQ)
+    THEN `2 EXP (a - b) = 2 EXP a` by IMP_RES_TAC LESS_EQUAL_ANTISYM
+    THEN A_FULL_SIMP_TAC [SUB_EQ_EQ_0,REDUCE_RULE (SPEC `2` EXP_INJECTIVE)]
+);
+
+val lem11 = (GEN_ALL o REWRITE_RULE [EXP,GSYM NOT_LESS_EQUAL])
+              (MATCH_MP TWOEXP_MONO (DECIDE (Term `h < SUC h`)));
+
+val TWOEXP_LT_EQ1 = prove(
+  `!n. 2 EXP n <= 1 ==> (2 EXP n = 1)`,
+  REPEAT STRIP_TAC THEN ASSUME_TAC (SPEC `n` ZERO_LT_TWOEXP) THEN DECIDE_TAC
+);
+
+(* |- !n x. ASRw (SUC x) n = ASR_ONEw (ASRw x n) *)
+val ASR_LEM = GEN_ALL (RIGHT_REWRITE_RULE [GSYM ASRw_def]
+                 (REWRITE_CONV [ASRw_def,FUNPOW_THM2] ``ASRw (SUC x) n``));
+
+val ASR_THM = store_thm("ASR_THM",
+  `!x n. ASRw x (wn n) =
+           let x' = MIN HB x in
+           let s = BITS HB x' n in
+             wn (if MSB n then 2 EXP WL - 2 EXP (WL - x') + s else s)`,
+  Induct_on `x`
+    THEN REPEAT STRIP_TAC
+    THENL [
+      A_RW_TAC [ASRw_def,FUNPOW,MIN_DEF,SYM MODw_THM,MODw_ELIM],
+      POP_ASSUM
+        (fn th => S_RW_TAC [th,REDUCE_RULE (SPEC `F` SET_def),lem3,lem7,
+                            lem,lem2,MIN_DEF,ASR_LEM,ASR_ONE_EVAL,ASR_ONE_def])
+        THEN A_FULL_SIMP_TAC [BITS_ZERO,lem9,SET_def]
+        THEN ASM_A_SIMP_TAC [lem8c,lem4,BITS_ZERO,WL_SUB_HB,WL_SUB_SUC_X]
+        THENL [
+          RW_TAC arithr_ss [WL_def,SUB_RIGHT_ADD,EXP,EXP_1,TWOEXP_LT_EQ1],
+          `x = HB` by DECIDE_TAC
+            THEN RW_TAC arithr_ss [WL_def,SUB_RIGHT_ADD,EXP,EXP_1,TWOEXP_LT_EQ1],
+          RW_TAC arithr_ss [WL_def,SUB_RIGHT_ADD,EXP,EXP_SUB_LESS_EQ]
+            THEN IMP_RES_TAC lem10
+            THEN A_FULL_SIMP_TAC [lem11]
+            THEN REWRITE_TAC [TIMES2]
+            THEN ONCE_REWRITE_TAC [DECIDE (Term `a + b + c = a + c + b`)]
+            THEN REWRITE_TAC [ADD_SUB]
+        ]
+    ]
+);
+
+(* ------------
 val LESS_SUC_EXP = prove(
   `!a b. a < 2 EXP SUC b ==> a DIV 2 < 2 EXP b`,
-  RW_TAC arith_ss [EXP,SYM (REDUCE_RULE (SPECL [`a DIV 2`,`2 EXP i`,`1`] LESS_MULT_MONO)),
-                   DIV_MULT_THM2,SUB_RIGHT_LESS,ZERO_LT_TWOEXP]
+  A_RW_TAC [EXP,SYM (REDUCE_RULE (SPECL [`a DIV 2`,`2 EXP i`,`1`] LESS_MULT_MONO)),
+            DIV_MULT_THM2,SUB_RIGHT_LESS,ZERO_LT_TWOEXP]
 );
 
 val INw_RSHIFT = store_thm("INw_RSHIFT",
@@ -1138,11 +1307,11 @@ val INw_RSHIFT = store_thm("INw_RSHIFT",
             THEN ASM_SIMP_TAC std_ss [GSYM SUB_LEFT_LESS,WL_def,EXP,TIMES2,ADD_SUB]
             THEN POP_ASSUM (fn th => ASSUME_TAC (REWRITE_RULE [WL_def] (SPECL [`f`,`a`] th)))
             THEN IMP_RES_TAC LESS_SUC_EXP,
-          FULL_SIMP_TAC arith_ss [SET_def,INw_def]
+          A_FULL_SIMP_TAC [SET_def,INw_def]
             THEN Cases_on `0 < FUNPOW (\x. x DIV 2 + (if f x then 2 EXP HB else 0)) n (MODw a)`
             THENL [
               IMP_RES_TAC DIV_LESS
-                THEN POP_ASSUM (fn th => ASSUME_TAC (SIMP_RULE std_ss [DECIDE(Term`1 < 2`)] (SPEC `2` th)))
+                THEN POP_ASSUM (fn th => ASSUME_TAC (SIMP_RULE std_ss [DECIDE `1 < 2`] (SPEC `2` th)))
                 THEN PAT_ASSUM `!f a.  FUNPOW (\x. x DIV 2 + (if f x then 2 EXP HB else 0)) n
                                 (MODw a) < 2 EXP WL` (fn th => ASSUME_TAC (SPECL [`f`,`a`] th))
                 THEN IMP_RES_TAC LESS_TRANS,
@@ -1181,6 +1350,7 @@ val ROR_EVAL = store_thm("ROR_EVAL",
                                    GSYM ADD_EVAL,ROR_ONE_def,LSR_ONE_def,MODw_ELIM,TOw_IDEM]
     ]
 );
+------------ *)
 
 (* -------------------------------------------------------- *)
 
@@ -1224,9 +1394,9 @@ val RRX_EVAL2 = save_thm("RRX_EVAL2",
 val LSB_EVAL2 = save_thm("LSB_EVAL2",GEN_ALL (REWRITE_RULE [LSB_ODD] LSB_EVAL));
 val MSB_EVAL2 = save_thm("MSB_EVAL2",GEN_ALL (REWRITE_RULE [MSB_def,HB_def] MSB_EVAL));
 
-val OR_EVAL2 = save_thm("OR_EVAL2",GEN_ALL (SIMP_RULE std_ss [OR_def,THE_WL] OR_EVAL));
-val AND_EVAL2 = save_thm("AND_EVAL2",GEN_ALL (SIMP_RULE std_ss [AND_def,THE_WL] AND_EVAL));
-val EOR_EVAL2 = save_thm("EOR_EVAL2",GEN_ALL (SIMP_RULE std_ss [EOR_def,THE_WL] EOR_EVAL));
+val OR_EVAL2  = save_thm("OR_EVAL2",GEN_ALL (SIMP_RULE bool_ss [OR_def,THE_WL] OR_EVAL));
+val AND_EVAL2 = save_thm("AND_EVAL2",GEN_ALL (SIMP_RULE bool_ss [AND_def,THE_WL] AND_EVAL));
+val EOR_EVAL2 = save_thm("EOR_EVAL2",GEN_ALL (SIMP_RULE bool_ss [EOR_def,THE_WL] EOR_EVAL));
 
 (* -------------------------------------------------------- *)
 
@@ -1237,52 +1407,51 @@ val BITWISE_EVAL2 = store_thm("BITWISE_EVAL2",
                       (if op (ODD x) (ODD y) then 1 else 0)`,
   REPEAT STRIP_TAC
     THEN Cases_on `n = 0`
-    THEN ASM_SIMP_TAC std_ss [BITWISE_def]
-    THEN RULE_ASSUM_TAC (REWRITE_RULE [NOT_ZERO_LT_ZERO])
-    THEN IMP_RES_TAC LESS_ADD_1
-    THEN FULL_SIMP_TAC arith_ss [GSYM ADD1,BITWISE_EVAL,SET_def,EXP,LSB_ODD]
+    THEN ASM_REWRITE_TAC [BITWISE_def]
+    THEN IMP_RES_TAC NOT_ZERO_ADD1
+    THEN A_FULL_SIMP_TAC [BITWISE_EVAL,SET_def,EXP,LSB_ODD]
 );
 
 (* -------------------------------------------------------- *)
 
 val BITSwLT_THM = store_thm("BITSwLT_THM",
   `!h l n. BITSw h l n < 2 EXP (SUC h-l)`,
-  RW_TAC std_ss [BITSLT_THM,BITSw_def]
+  B_RW_TAC [BITSLT_THM,BITSw_def]
 );
 
 val BITSw_COMP_THM = store_thm("BITSw_COMP_THM",
   `!h1 l1 h2 l2 n. h2 + l1 <= h1 ==> (BITS h2 l2 (BITSw h1 l1 n) = BITSw (h2+l1) (l2+l1) n)`,
-  RW_TAC std_ss [BITSw_def,BITS_COMP_THM]
+  B_RW_TAC [BITSw_def,BITS_COMP_THM]
 );
  
 val BITSw_DIV_THM = store_thm("BITSw_DIV_THM",
   `!h l n x. (BITSw h l x) DIV 2 EXP n = BITSw h (l + n) x`,
-  RW_TAC std_ss [BITSw_def,BITS_DIV_THM]
+  B_RW_TAC [BITSw_def,BITS_DIV_THM]
 );
 
 val BITw_THM = store_thm("BITw_THM",
   `!b n. BITw b n = (BITSw b b n = 1)`,
-  RW_TAC std_ss [BITSw_def,BITw_def,BIT_def]
+  B_RW_TAC [BITSw_def,BITw_def,BIT_def]
 );
  
 val SLICEw_THM = store_thm("SLICEw_THM",
   `!n h l. SLICEw h l n = BITSw h l n * 2 EXP l`,
-  RW_TAC std_ss [SLICEw_def,BITSw_def,SLICE_THM]
+  B_RW_TAC [SLICEw_def,BITSw_def,SLICE_THM]
 );
 
 val BITS_SLICEw_THM = store_thm("BITS_SLICEw_THM",
   `!h l n. BITS h l (SLICEw h l n) = BITSw h l n`,
-  RW_TAC std_ss [SLICEw_def,BITSw_def,BITS_SLICE_THM]
+  B_RW_TAC [SLICEw_def,BITSw_def,BITS_SLICE_THM]
 );
 
 val SLICEw_ZERO_THM = store_thm("SLICEw_ZERO_THM",
   `!n h. SLICEw h 0 n = BITSw h 0 n`,
-  RW_TAC arithr_ss [SLICEw_THM]
+  R_RW_TAC [SLICEw_THM]
 );
  
 val SLICEw_COMP_THM = store_thm("SLICEw_COMP_THM",
   `!h m l a. (SUC m) <= h /\ l <= m ==> (SLICEw h (SUC m) a + SLICEw m l a = SLICEw h l a)`,
-  RW_TAC std_ss [SLICEw_def,SLICE_COMP_THM]
+  B_RW_TAC [SLICEw_def,SLICE_COMP_THM]
 );
 
 (* -------------------------------------------------------- *)
